Process_Epoch_O_Specs.thy
@@ -1,5 +1,5 @@
 theory Process_Epoch_O_Specs
-imports ProcessEpoch_O
+imports ProcessEpoch_O sqrt_proof
 begin
 
 locale extended_hl_pre =  extended_vc  + hoare_logic
@@ -49,7 +49,7 @@ lemma sub_wp[wp]: "hoare_triple (lift (P (n - m))) (c (n - m)) Q \<Longrightarro
    apply (simp only: Let_unfold)
    apply (wp, clarsimp simp: bindCont_return')
   apply (safe)
-  apply (simp add: word_sub_le_iff)
+  by (simp add: word_sub_le_iff)
   apply (erule notE)
   apply (clarsimp simp: lift_def)
   using word_sub_le_iff by blast
@@ -258,8 +258,7 @@ lemma sum_list_wp[wp]: "hoare_triple (lift (P (sum_list xs))) (f (sum_list xs)) 
     hoare_triple (lift (\<lambda>s. (sum_list (map unat xs)) \<le> 2^64 - 1 \<and> ((sum_list (map unat xs)) \<le> 2^64 - 1 \<longrightarrow> P (sum_list xs) s))) (do {b <- safe_sum xs; f b}) Q"
   apply ( rule hoare_assert_stateI, clarsimp)
   apply (subst safe_sum_distinct_wb, clarsimp)
-  apply (clarsimp simp: lift_def)
-  apply (clarsimp simp: bindCont_return)
+  apply (clarsimp)
   apply (rule hoare_weaken_pre, assumption)
   apply (clarsimp)
   done
@@ -274,7 +273,7 @@ lemma maps_to_is_valid:"(maps_to l v \<and>* R) s \<Longrightarrow> valid (l) (S
   sorry
 
 lemma valid_validator_some_simp[simp]: 
-"valid validators (Some xs) = (let ys = Invariants.var_list_inner xs in sum_list (map (unat o effective_balance_f) ys) < 2^(64) \<and> distinct ys \<and> length ys < 2^64 )"
+"valid validators (Some xs) = (let ys = Invariants.var_list_inner xs in sum_list (map (unat o Validator.effective_balance_f) ys) < 2^(64) \<and> distinct ys \<and> length ys < 2^64 )"
   apply (clarsimp simp: validators_def)
   sorry
   
@@ -363,10 +362,22 @@ lemma index_in_length_in_set[intro!]: "xb < var_list_len v \<Longrightarrow> loc
   apply (case_tac v; clarsimp)
   by (simp add: unat_less_helper)
 
+find_theorems select
 
-lemma get_total_balance_wp[wp]:"(\<And>x xs (v :: Validator VariableList). distinct xs \<Longrightarrow> list.set xs = S \<Longrightarrow> x = max (EFFECTIVE_BALANCE_INCREMENT config) (sum_list (map (effective_balance_f \<circ> unsafe_var_list_index v) xs)) \<Longrightarrow>
+
+lemma select_wp_lift[wp]: "(\<And>x. x \<in> P \<Longrightarrow> hoare_triple (lift (pre x)) (f x) Q) \<Longrightarrow> hoare_triple (lift (\<lambda>s. \<forall>x\<in>P. pre x s)) (do {x <- select P; f x}) Q"
+  apply (clarsimp simp: select_def bindCont_def hoare_triple_def run_def)
+  apply (subst Sup_le_iff)
+  apply (clarsimp)
+  apply (atomize, erule allE, drule mp, assumption)
+  apply (erule order_trans)
+  apply (rule seq_mono_left)
+  by (subst assert_iso[symmetric], clarsimp)
+
+
+lemma get_total_balance_wp[wp]:"(\<And>x xs (v :: Validator VariableList). distinct xs \<Longrightarrow> list.set xs = S \<Longrightarrow> x = max (EFFECTIVE_BALANCE_INCREMENT config) (sum_list (map (Validator.effective_balance_f \<circ> unsafe_var_list_index v) xs)) \<Longrightarrow>
     hoare_triple (lift (P x)) (f x) Q) 
-  \<Longrightarrow> hoare_triple (lift ((maps_to validators v \<and>* (maps_to validators v \<longrightarrow>* (\<lambda>s. (\<forall>x\<in>S. x < var_list_len v) \<and>  ((\<forall>x\<in>S. x < var_list_len v) \<longrightarrow> (\<forall>xs\<in>lists_of S. P (max (EFFECTIVE_BALANCE_INCREMENT config) (sum_list (map (effective_balance_f \<circ> unsafe_var_list_index v) xs))) s)  )))) ))
+  \<Longrightarrow> hoare_triple (lift ((maps_to validators v \<and>* (maps_to validators v \<longrightarrow>* (\<lambda>s. (\<forall>x\<in>S. x < var_list_len v) \<and>  ((\<forall>x\<in>S. x < var_list_len v) \<longrightarrow> (\<forall>xs\<in>lists_of S. P (max (EFFECTIVE_BALANCE_INCREMENT config) (sum_list (map (Validator.effective_balance_f \<circ> unsafe_var_list_index v) xs))) s)  )))) ))
    (do {b <- get_total_balance S; f b}) Q"
   apply (clarsimp simp: get_total_balance_def, rule hoare_weaken_pre)
    apply (wp)
@@ -583,6 +594,1464 @@ lemma "hoare_triple (lift (maps_to beacon_slots b \<and>* maps_to previous_epoch
  apply (sep_frule (direct) maps_to_is_valid[where l=validators])
      apply (clarsimp simp: Let_unfold)
   apply (case_tac v; clarsimp)
+  done
+
+lemma div_wp_lift: "hoare_triple (lift (P (n div m))) (c (n div m)) Q \<Longrightarrow>
+  hoare_triple (lift (\<lambda>s. m \<noteq> 0 \<and> (m \<noteq> 0 \<longrightarrow>  (P ( n div m)) s))) 
+(do {x <- (word_unsigned_div n m); c x}) Q"
+  apply (rule hoare_weaken_pre)
+   apply (unfold word_unsigned_div_def, wp)
+  apply (clarsimp simp: bindCont_return')
+  apply (clarsimp simp: lift_def)
+  done
+
+find_theorems name:div_wp
+
+lemma [simp]: "CHURN_LIMIT_QUOTIENT config \<noteq> 0" sorry
+
+lemma get_validator_churn_limit_fast_spec: "hoare_triple (\<lless>num_active_validators \<mapsto>\<^sub>l n \<and>* R\<then>) get_validator_churn_limit_fast (lift (num_active_validators \<mapsto>\<^sub>l n \<and>* R))"
+  apply (clarsimp simp: get_validator_churn_limit_fast_def, rule hoare_weaken_pre)
+   apply (wp)
+   apply (rule div_wp_lift)
+   apply (rule return_wp)
+  apply (clarsimp)
+  apply (sep_solve)
+  done
+
+lemma get_validator_churn_limit_fast_wp[wp]: "(\<And>x. hoare_triple (lift (P x)) (c x) Q) \<Longrightarrow> 
+     hoare_triple (\<lless>num_active_validators \<mapsto>\<^sub>l n \<and>* (num_active_validators \<mapsto>\<^sub>l n \<longrightarrow>* P (max (MIN_PER_EPOCH_CHURN_LIMIT config) (n div CHURN_LIMIT_QUOTIENT config)))\<then>) 
+      (bindCont get_validator_churn_limit_fast c) (Q)"
+  apply (clarsimp simp: get_validator_churn_limit_fast_def, rule hoare_weaken_pre)
+   apply (wp)
+   apply (rule div_wp_lift)
+  apply (fastforce)
+  apply (clarsimp)
+  apply (sep_cancel)+
+  done
+
+lemma get_validator_churn_limit_spec: "hoare_triple (\<lless>beacon_slots \<mapsto>\<^sub>l v \<and>* validators \<mapsto>\<^sub>l vs \<and>*  R\<then>) get_validator_churn_limit (lift (beacon_slots \<mapsto>\<^sub>l v \<and>* validators \<mapsto>\<^sub>l vs \<and>* R))"
+  apply (clarsimp simp: get_validator_churn_limit_def, rule hoare_weaken_pre)
+   apply (wp)
+   apply (rule div_wp_lift)
+   apply (rule return_wp)
+  apply (clarsimp)
+  apply (sep_cancel)+
+  done
+
+lemma get_validator_churn_limit_spec': "(\<And>x. hoare_triple (lift (P x)) (c x) Q) \<Longrightarrow>
+   hoare_triple (\<lless>beacon_slots \<mapsto>\<^sub>l v \<and>* validators \<mapsto>\<^sub>l vs \<and>* (beacon_slots \<mapsto>\<^sub>l v \<and>* validators \<mapsto>\<^sub>l vs \<longrightarrow>* P (max (MIN_PER_EPOCH_CHURN_LIMIT config) (word_of_nat (length (active_validator_indices (slot_to_epoch config v) vs)) div CHURN_LIMIT_QUOTIENT config))) \<then>) (bindCont get_validator_churn_limit c) (Q)"
+  apply (clarsimp simp: get_validator_churn_limit_def, rule hoare_weaken_pre)
+   apply (wp)
+   apply (rule div_wp_lift)
+  apply (assumption)
+  apply (clarsimp)
+  apply (sep_cancel)+
+  apply (sep_mp)
+  apply (sep_cancel)+
+  done
+
+lemma [simp]: "\<lless>\<lambda>s. P\<then> = (\<lambda>s. P)" 
+  apply (intro ext, clarsimp simp: lift_def)  
+  apply (safe)
+  apply (rule_tac x="id_p" in exI)
+  by simp
+
+lemma add_wp[wp]: "hoare_triple (lift (P (n + m))) (c (n + m)) Q \<Longrightarrow>
+  hoare_triple (lift (\<lambda>s. n \<le> n + m \<and> (n \<le> n + m \<longrightarrow> P (n + m) s))) 
+(do {x <- (word_unsigned_add n  m); c x}) Q"
+  apply (rule hoare_weaken_pre)
+   apply (clarsimp simp:  word_unsigned_add_def )
+   apply (simp only: Let_unfold)
+   apply (wp, clarsimp simp: bindCont_return')
+  done
+
+lemma mod_wp[wp]: "hoare_triple (lift (P (n mod m))) (c (n mod m)) Q \<Longrightarrow>
+  hoare_triple (lift (\<lambda>s. m \<noteq> 0 \<and> (m \<noteq> 0 \<longrightarrow> P (n mod m) s)))
+(do {x <- (n .% m); c x}) Q"
+  apply (rule hoare_weaken_pre)
+   apply (unfold word_unsigned_mod_def)
+   apply wp
+  apply fastforce
+  done
+
+find_theorems name:if_wp
+
+thm wp
+
+lemma when_wp[wp]: 
+  "(B \<Longrightarrow> hoare_triple  ( lift S) ( bindCont P c) R) \<Longrightarrow> (\<not>B \<Longrightarrow> hoare_triple ( lift S') (c ()) R) \<Longrightarrow>
+   hoare_triple ( lift (if B then S else S'))  (do {x <- (when B P); c x}) R"
+  apply (clarsimp split: if_splits)
+  done
+
+definition "next_epoch b_slots \<equiv> epoch_to_u64 (slot_to_epoch config b_slots) + 1"
+
+lemma SLOTS_PER_EPOCH_ATLEAST[simp]: "1 < SLOTS_PER_EPOCH config" sorry
+lemma EPOCHS_PER_ETH1_VOTING_PERIOD_ATLEAST[simp]: "EPOCHS_PER_ETH1_VOTING_PERIOD config \<noteq> 0" sorry
+
+lemma process_eth1_data_reset: "hoare_triple (lift (beacon_slots \<mapsto>\<^sub>l b \<and>* eth1_data_votes \<mapsto>\<^sub>l data_votes \<and>*  R))
+         process_eth1_data_reset 
+      (lift (beacon_slots \<mapsto>\<^sub>l b \<and>* 
+   eth1_data_votes \<mapsto>\<^sub>l (if (next_epoch b) mod (EPOCHS_PER_ETH1_VOTING_PERIOD config) = 0 then (VariableList []) else data_votes) \<and>*  R))"
+  apply (unfold process_eth1_data_reset_def epoch_unsigned_add_def, rule hoare_weaken_pre)
+   apply (wp)
+  apply (safe)
+  apply (sep_cancel)+
+  apply (intro conjI impI)
+    apply (clarsimp)
+    apply (clarsimp simp: slot_to_epoch_def)
+    apply (subgoal_tac "SLOTS_PER_EPOCH config > 1")
+     apply (metis bits_div_0 div_less_dividend_word less_is_non_zero_p1 lt1_neq0 olen_add_eqv word_less_1 zero_neq_one)
+    apply (clarsimp)
+  apply (clarsimp)
+  apply (clarsimp simp: next_epoch_def)
+  by (sep_cancel)+
+
+thm get_previous_epoch_wp
+
+definition "previous_epochs bs = {e. e \<le> previous_epoch (slot_to_epoch config bs)}"
+
+lemma raw_epoch_simp: "raw_epoch = epoch_to_u64"
+  by (intro ext, case_tac x; clarsimp)
+
+lemma get_finality_delay_wp[wp]:
+"hoare_triple (lift (P (raw_epoch (previous_epoch (slot_to_epoch config bs)) - raw_epoch (epoch_f f_c))))
+       (c ((raw_epoch (previous_epoch (slot_to_epoch config bs)) - raw_epoch (epoch_f f_c)))) R \<Longrightarrow>
+           hoare_triple (lift (\<lambda>s. epoch_f f_c \<in> previous_epochs bs \<and> (epoch_f f_c \<in> previous_epochs bs \<longrightarrow>
+           (beacon_slots \<mapsto>\<^sub>l bs \<and>* finalized_checkpoint \<mapsto>\<^sub>l f_c \<and>* (beacon_slots \<mapsto>\<^sub>l bs \<and>*  finalized_checkpoint \<mapsto>\<^sub>l f_c \<longrightarrow>* P (raw_epoch (previous_epoch (slot_to_epoch config bs)) - raw_epoch (epoch_f f_c)))) s) ) ) 
+(bindCont get_finality_delay c) ( R )"
+  apply (unfold get_finality_delay_def, rule hoare_weaken_pre)
+   apply (wp)
+   apply (clarsimp simp: raw_epoch_simp)
+   apply (erule hoare_eqI')
+  apply (clarsimp)
+  apply (sep_cancel)+
+  apply (intro conjI impI)
+  apply (clarsimp)
+   apply (clarsimp simp: previous_epochs_def)
+  using less_eq_Epoch_def apply blast
+   apply (clarsimp)
+   apply (sep_mp)
+   apply (clarsimp simp: raw_epoch_simp)
+   apply (clarsimp simp: raw_epoch_simp)
+  done
+
+
+abbreviation (input) "sep_wp pre post P \<equiv> (lift (pre \<and>* (post \<longrightarrow>* P)))"
+
+lemma lift_pure_conj[simp]: "lift (\<lambda>s. P \<and> Q s) s = (P \<and> lift Q s)"
+  by (clarsimp simp: lift_def)
+
+lemma lift_pure_imp[simp]: "lift (\<lambda>s. P \<longrightarrow> Q s) s = (P \<longrightarrow> lift Q s)"
+  apply (clarsimp simp: lift_def)
+  apply (safe, blast)
+  apply (rule_tac x=id_p in exI)
+   apply (clarsimp)
+  apply (blast)
+  done
+
+
+schematic_goal is_in_activity_leak[wp]:
+ "hoare_triple (lift (pre ?x)) (c ?x) post \<Longrightarrow>
+   hoare_triple
+    (sep_wp (beacon_slots \<mapsto>\<^sub>l b_s \<and>* finalized_checkpoint \<mapsto>\<^sub>l c_f)
+  (beacon_slots \<mapsto>\<^sub>l b_s \<and>* finalized_checkpoint \<mapsto>\<^sub>l c_f)
+ (\<lambda>s. Checkpoint.epoch_f c_f \<in> previous_epochs b_s \<and> (Checkpoint.epoch_f c_f \<in> previous_epochs b_s \<longrightarrow> pre ?x s)))
+  (bindCont is_in_inactivity_leak c) post"
+  apply (unfold is_in_inactivity_leak_def, rule hoare_weaken_pre)
+   apply (wp)
+  apply (rule lift_mono')
+  apply (clarsimp)
+  apply (intro conjI impI)
+   apply (clarsimp simp: sep_conj_assoc)
+   defer
+   apply (clarsimp simp: sep_conj_assoc)
+   apply (sep_cancel)+
+  apply (sep_mp)
+   apply (clarsimp)
+  apply (sep_mp)
+  apply (clarsimp)
+  done
+
+lemma epoch_always_bounded[simp]: "epoch_to_u64 (slot_to_epoch config v) \<le> epoch_to_u64 (slot_to_epoch config v) + 1"
+  apply (clarsimp simp: slot_to_epoch_def)
+  by (metis (no_types, opaque_lifting) SLOTS_PER_EPOCH_ATLEAST add.commute
+             bits_div_0 div_less_dividend_word inc_i le_no_overflow lt1_neq0
+                                    verit_comp_simplify1(2) word_le_not_less)
+
+
+lemma subst_in_impl: "(x = y \<longrightarrow> f y) = (x = y \<longrightarrow> f x)"
+  by (safe)
+
+lemma hoare_eqI': "hoare_triple (lift (P x)) (f x) Q \<Longrightarrow> hoare_triple (lift (\<lambda>s. v = x \<and> (v = x \<longrightarrow> P v s))) (f v) Q"
+  apply (rule hoare_assert_stateI)
+  apply (clarsimp)
+  apply (clarsimp simp: lift_def)
+  apply (erule hoare_weaken_pre)
+  apply (clarsimp simp: lift_def)
+  apply (blast)
+  done
+
+lemma hoare_eqI'': "hoare_triple (lift (P x v)) (f x) Q \<Longrightarrow> hoare_triple (lift (\<lambda>s. v = x \<and> (v = x \<longrightarrow> P x v s))) (f v) Q"
+  apply (rule hoare_assert_stateI)
+  apply (clarsimp)
+  apply (clarsimp simp: lift_def)
+  apply (erule hoare_weaken_pre)
+  apply (clarsimp simp: lift_def)
+  apply (blast)
+  done
+
+schematic_goal new_state_context_wp[simplified subst_in_impl, wp]: 
+ "hoare_triple (lift (pre ?x)) (c ?x) post \<Longrightarrow> hoare_triple (lift ?P) (bindCont new_state_context c) (post)"
+  apply (unfold new_state_context_def epoch_unsigned_add_def, rule hoare_weaken_pre)
+   apply (wp)
+  apply (erule hoare_eqI')
+  apply (clarsimp simp: subst_in_impl)
+  apply (sep_cancel)+
+  done
+
+definition "safe_mul m n \<equiv> if (m = 0 \<or> n = 0) then True else (m * n div n = m)"
+
+lemma fail_wp[wp]: "\<lblot>lift \<bottom>\<rblot> bindCont fail c \<lblot>Q\<rblot>"
+  apply (rule hoare_weaken_pre, wp)
+  apply (clarsimp simp: lift_def)
+  done
+
+thm mul_wp
+
+lemma mul_wp[wp]: "hoare_triple (lift (P (n * m))) (c (n * m)) Q \<Longrightarrow>
+  hoare_triple (lift (\<lambda>s. safe_mul m n  \<and> (safe_mul m n  \<longrightarrow> P (n * m) s))) 
+(do {x <- (word_unsigned_mul n m); c x}) Q"
+  apply (rule hoare_weaken_pre)
+   apply (unfold  word_unsigned_mul_def )
+   apply (simp only: Let_unfold)
+   apply (rule if_wp, simp)
+    apply (fastforce)
+   apply (rule if_wp, simp)
+   apply (wp)
+  apply (clarsimp simp: safe_mul_def)
+  apply (intro conjI impI; clarsimp?)
+  by (simp add: mult.commute)
+
+lemma div_wp[wp]: "hoare_triple (lift (P (n div m))) (c (n div m)) Q \<Longrightarrow>
+  hoare_triple (lift (\<lambda>s. m \<noteq> 0 \<and> (m \<noteq> 0 \<longrightarrow> P ( n div m) s))) 
+(do {x <- (word_unsigned_div n m); c x}) Q"
+  apply (rule hoare_weaken_pre)
+   apply (unfold word_unsigned_div_def, wp)
+   apply (clarsimp simp: bindCont_return')
+  done
+
+lemma slashings_wf: "(slashings \<mapsto>\<^sub>l ss \<and>* R) s \<Longrightarrow> 
+sum_list (map unat (local.vector_inner ss)) \<le> 2 ^ 64 - 1 \<and> 
+PROPORTIONAL_SLASHING_MULTIPLIER_BELLATRIX = sum_list (local.vector_inner ss) *
+PROPORTIONAL_SLASHING_MULTIPLIER_BELLATRIX div sum_list (local.vector_inner ss)"
+  sorry
+
+schematic_goal new_slashings_context_wp[wp]: 
+  "hoare_triple (lift (P x)) (c x) Q \<Longrightarrow> hoare_triple (lift (slashings \<mapsto>\<^sub>l ss \<and>* ?R)) (bindCont (new_slashings_context st_ctxt pbc) c) ( Q)"
+  apply (clarsimp simp: new_slashings_context_def, rule hoare_weaken_pre , wp)
+   apply (erule hoare_eqI')
+  apply (clarsimp)
+  apply (frule slashings_wf)
+  apply (erule sep_conj_impl, assumption)
+  apply (clarsimp)
+  apply (assumption)
+  done
+
+
+schematic_goal new_activation_queue_wp[wp]:
+  "hoare_triple (lift (P x)) (c x) Q \<Longrightarrow> 
+   hoare_triple (lift (beacon_slots \<mapsto>\<^sub>l b_s \<and>* validators \<mapsto>\<^sub>l vs \<and>* 
+  (validators \<mapsto>\<^sub>l vs \<and>* beacon_slots \<mapsto>\<^sub>l b_s \<longrightarrow>*
+    (\<lambda>sc. fold (\<lambda>(i, v) q. add_if_could_be_eligible_for_activation q i v (Epoch (next_epoch b_s))) (local.enumerate (local.var_list_inner vs)) (ActivationQueue.fields []) = x \<and>
+(fold (\<lambda>(i, v) q. add_if_could_be_eligible_for_activation q i v (Epoch (next_epoch b_s))) (local.enumerate (local.var_list_inner vs)) (ActivationQueue.fields []) = x \<longrightarrow> P x sc))) ))
+   (bindCont new_activation_queue c) Q"
+  apply (clarsimp simp: new_activation_queue_def epoch_unsigned_add_def, rule hoare_weaken_pre, wp)
+   apply (erule hoare_eqI')
+  apply (clarsimp)
+  apply (fold next_epoch_def)
+  apply (sep_cancel)+
+  apply (sep_mp, clarsimp)
+  done
+
+abbreviation "map_varlist f xs \<equiv> map f (local.var_list_inner xs)"
+
+definition "frequency_map xs = Some(0 := None) o of_nat o (count_list xs)"
+
+lemma exit_cache_eq_iff: "(x :: ExitCache) = y \<longleftrightarrow> exit_epoch_counts_f x = exit_epoch_counts_f y"
+  by (case_tac x; case_tac y; clarsimp)
+
+lemma  new_exit_cache_wp[wp]: "
+  hoare_triple (lift (P x)) (c x) Q \<Longrightarrow> 
+  hoare_triple (lift (validators \<mapsto>\<^sub>l vs \<and>*
+                     (validators \<mapsto>\<^sub>l vs \<longrightarrow>* 
+                       (\<lambda>s. exit_epoch_counts_f x = frequency_map (map_varlist exit_epoch_f vs) \<and> 
+                       (exit_epoch_counts_f x = frequency_map (map_varlist exit_epoch_f vs) \<longrightarrow> P x s)))))
+                (bindCont new_exit_cache c) Q"
+  apply (clarsimp simp: new_exit_cache_def Let_unfold, rule hoare_weaken_pre, wp)
+     apply (erule hoare_eqI')
+  apply (clarsimp)
+  apply (sep_cancel)+
+  apply (intro conjI impI)
+  apply (sep_mp)
+  apply (clarsimp)
+   apply (clarsimp simp: frequency_map_def exit_cache_eq_iff ExitCache.defs)
+   apply (intro ext, clarsimp)
+  apply (sep_mp, clarsimp)
+  done
+
+
+lemma mapM_wp'':
+  assumes c_wp: "\<And>(f :: 'e \<Rightarrow> ('f, 'a) cont) x P Q.  (\<And>xs. hoare_triple (lift (P (g x))) (f (g x)) ( Q)) \<Longrightarrow> hoare_triple (lift (pre x)) (do { b <- c x; f b}) Q"  
+shows "  (\<And>x y. hoare_triple (lift (P x)) (f y) Q) \<Longrightarrow>   hoare_triple (lift (\<lambda>s. (\<forall>x\<in>list.set xs. pre x s) \<and> ((\<forall>x\<in>list.set xs. pre x s) \<longrightarrow> P (map g xs) s))) (do {vs <- mapM c (xs :: 'd list) ; (f :: 'e list \<Rightarrow> ('f, 'a) cont) (vs )}) Q"
+  apply (induct xs arbitrary: f)
+   apply (simp)
+  apply (clarsimp)
+  apply (rule hoare_weaken_pre)
+  apply (clarsimp simp: bindCont_assoc[symmetric])
+   apply (rule c_wp)
+  defer
+    apply (clarsimp)
+  defer
+  apply (atomize)
+  apply (erule_tac x="(\<lambda>aa. f (g a # aa))" in allE)
+  apply (drule mp)
+   apply (clarsimp)
+  apply (fastforce)
+  done
+
+thm mapM_wp
+
+term "foldr (\<lambda>x R. pre' R x) xs"
+
+lemma mapM_wp_foldr:
+  assumes c_wp: "\<And>(f :: 'e \<Rightarrow> ('f, 'a) cont) x P Q. (\<And>x. hoare_triple (lift (P)) (f x) (Q)) \<Longrightarrow> hoare_triple (lift (pre P x)) (do { b <- c x; f b}) Q"  
+shows " (\<And>x. hoare_triple (lift (P)) (f x) Q) \<Longrightarrow>   hoare_triple (lift (foldr (\<lambda>x R. pre R x) xs P )) (do {vs <- mapM c (xs :: 'd list) ; (f :: 'e list \<Rightarrow> ('f, 'a) cont) (vs )}) Q"
+  apply (induct xs arbitrary: f; clarsimp)
+  by (metis (no_types, lifting) bindCont_assoc c_wp return_triple')
+
+lemma mapM_wp':
+  assumes c_wp: "\<And>(f :: 'e \<Rightarrow> ('f, 'a) cont) x P Q. hoare_triple (lift P) (f (g x)) ( Q) \<Longrightarrow> hoare_triple (lift (pre P x)) (do { b <- c x; f b}) Q"  
+  assumes pre_mono: "(\<And>x P Q s . (P s  \<Longrightarrow> Q s) \<Longrightarrow>  (pre P x) s \<Longrightarrow>  (pre Q x) s  )"
+shows " hoare_triple (lift P) (f (map g xs)) Q \<Longrightarrow>   hoare_triple (lift (\<lambda>s. (\<Sqinter>x\<in>(list.set xs). pre P x) s \<and> ((\<Sqinter>x\<in>(list.set xs). pre P x) s \<longrightarrow> P s))) (do {vs <- mapM c (xs :: 'd list) ; (f :: 'e list \<Rightarrow> ('f, 'a) cont) (vs )}) Q"
+  apply (induct xs arbitrary: f; clarsimp)
+  apply (atomize)
+  apply (clarsimp simp: bindCont_assoc[symmetric])
+  apply (rule hoare_weaken_pre)
+  apply (rule c_wp)
+  apply (erule allE)
+  apply (erule impE)
+   defer
+    apply (assumption)
+   apply (clarsimp)
+   apply (rule pre_mono[rotated], assumption)
+   apply (clarsimp)
+  
+  apply (clarsimp)
+  done
+
+lemma ebi_not_zero[intro]: "EFFECTIVE_BALANCE_INCREMENT config \<noteq> 0" sorry
+
+lemma brf_ebi_times_bounded[simp]: 
+      "EFFECTIVE_BALANCE_INCREMENT config * 
+       BASE_REWARD_FACTOR config div EFFECTIVE_BALANCE_INCREMENT config = 
+       BASE_REWARD_FACTOR config" sorry
+
+lemma sqrt_eq_zero_iff[simp]: "sqrt' x = 0 \<longleftrightarrow> x = 0"
+  by (metis (no_types, opaque_lifting) add_0 bits_div_by_1
+   comm_monoid_mult_class.mult_1 linorder_not_le lt1_neq0 
+       sqrt_induct sqrt_le sub_wrap word_not_simps(1))
+
+definition "mul_bound x y \<equiv> y = x * y div x"
+
+lemma safe_mul_commute: "safe_mul (x :: u64) y = safe_mul y x"
+  apply (clarsimp simp: safe_mul_def)
+  apply (safe)
+   apply (unat_arith, simp)
+   apply (metis (no_types, lifting) bot_nat_0.not_eq_extremum div_mult_le mult.commute
+        nonzero_mult_div_cancel_left order_le_less_trans unat_mult_lem unsigned_less)
+ apply (unat_arith, simp)
+   apply (metis (no_types, lifting) bot_nat_0.not_eq_extremum div_mult_le mult.commute
+        nonzero_mult_div_cancel_left order_le_less_trans unat_mult_lem unsigned_less)
+  done
+
+schematic_goal get_base_reward_fast_wp[wp]:
+ "hoare_triple (lift (P x)) (c x) Q \<Longrightarrow> hoare_triple (lift (\<lambda>s. total_active_balance_f pbc < total_active_balance_f pbc + 1 \<and>
+          (total_active_balance_f pbc < total_active_balance_f pbc + 1 \<longrightarrow>
+           total_active_balance_f pbc \<noteq> 0 \<and>
+           (total_active_balance_f pbc \<noteq> 0 \<longrightarrow>
+            safe_mul (effective_balance div EFFECTIVE_BALANCE_INCREMENT config) (EFFECTIVE_BALANCE_INCREMENT config * BASE_REWARD_FACTOR config div sqrt' (total_active_balance_f pbc)) \<and>
+            (safe_mul (effective_balance div EFFECTIVE_BALANCE_INCREMENT config) (EFFECTIVE_BALANCE_INCREMENT config * BASE_REWARD_FACTOR config div sqrt' (total_active_balance_f pbc)) \<longrightarrow>
+             effective_balance div EFFECTIVE_BALANCE_INCREMENT config * (EFFECTIVE_BALANCE_INCREMENT config * BASE_REWARD_FACTOR config div sqrt' (total_active_balance_f pbc)) = x \<and>
+             (effective_balance div EFFECTIVE_BALANCE_INCREMENT config * (EFFECTIVE_BALANCE_INCREMENT config * BASE_REWARD_FACTOR config div sqrt' (total_active_balance_f pbc)) = x \<longrightarrow> P x s ))))))
+        (bindCont (get_base_reward_fast effective_balance pbc) c) Q"
+  apply (clarsimp simp: get_base_reward_fast_def, rule hoare_weaken_pre, wp)
+   apply (clarsimp simp: get_base_reward_per_increment_fast_def, wp)
+   apply (erule hoare_eqI')
+  apply (clarsimp)
+  apply (intro conjI impI; clarsimp?)
+  using ebi_not_zero apply force
+   apply (metis brf_ebi_times_bounded mult.commute safe_mul_def)
+  using safe_mul_commute by blast
+
+lemma nonempty_ball_conj_lift: "S \<noteq> {} \<Longrightarrow> (\<forall>x\<in>S. P \<and> Q x) = (P \<and> (\<forall>x\<in>S. Q x))"
+  by (safe; clarsimp?)
+
+
+lemma nonempty_ball_imp_lift: "S \<noteq> {} \<Longrightarrow> (\<forall>x\<in>S. P \<longrightarrow> Q x) = (P \<longrightarrow> (\<forall>x\<in>S. Q x))"
+  by (safe; clarsimp?)
+
+lemma effective_balance_safe[simp]:
+ "MAX_EFFECTIVE_BALANCE \<le> MAX_EFFECTIVE_BALANCE + EFFECTIVE_BALANCE_INCREMENT config" sorry 
+
+lemma range_empty_iff: " (range x y z) = [] \<longleftrightarrow> (x \<ge> y) \<or> z = 0"
+  apply (case_tac z; clarsimp)
+  done 
+
+lemma start_in_valid_range[simp]: "range x y z \<noteq> [] \<Longrightarrow> x \<in> list.set (range x y z)"
+  apply (clarsimp simp: range_empty_iff)
+  by (case_tac z; clarsimp?)
+
+lemma EBI_ge_zero[intro]: "EFFECTIVE_BALANCE_INCREMENT config > 0" sorry
+
+schematic_goal compute_base_rewards_wp[wp]:
+ "(\<And>x. hoare_triple (lift (P x)) (c x) Q) \<Longrightarrow> 
+ hoare_triple 
+  (lift (progressive_balances_cache \<mapsto>\<^sub>l pbc \<and>* (progressive_balances_cache \<mapsto>\<^sub>l pbc \<longrightarrow>*
+        (\<lambda>s. total_active_balance_f pbc < total_active_balance_f pbc + 1 \<and>
+              (total_active_balance_f pbc < total_active_balance_f pbc + 1 \<longrightarrow>
+               total_active_balance_f pbc \<noteq> 0 \<and>
+               (total_active_balance_f pbc \<noteq> 0 \<longrightarrow>
+                (\<forall>f\<in>list.set (local.range 0 (unat (MAX_EFFECTIVE_BALANCE + EFFECTIVE_BALANCE_INCREMENT config)) (unat (EFFECTIVE_BALANCE_INCREMENT config))).
+                    safe_mul (word_of_nat f div EFFECTIVE_BALANCE_INCREMENT config) (EFFECTIVE_BALANCE_INCREMENT config * BASE_REWARD_FACTOR config div sqrt' (total_active_balance_f pbc)) \<and>
+                    (safe_mul (word_of_nat f div EFFECTIVE_BALANCE_INCREMENT config) (EFFECTIVE_BALANCE_INCREMENT config * BASE_REWARD_FACTOR config div sqrt' (total_active_balance_f pbc)) \<longrightarrow>
+                   
+                      P ((map (\<lambda>effective_balance.
+                        word_of_nat effective_balance div EFFECTIVE_BALANCE_INCREMENT config * (EFFECTIVE_BALANCE_INCREMENT config * BASE_REWARD_FACTOR config div sqrt' (total_active_balance_f pbc)))
+                       (local.range 0 (unat (MAX_EFFECTIVE_BALANCE + EFFECTIVE_BALANCE_INCREMENT config)) (unat (EFFECTIVE_BALANCE_INCREMENT config))))) s))))) ))) 
+       (bindCont compute_base_rewards c) Q"
+  apply (clarsimp simp: compute_base_rewards_def, rule hoare_weaken_pre, wp)
+  apply (rule mapM_wp'[where g="(\<lambda>effective_balance. of_nat effective_balance div EFFECTIVE_BALANCE_INCREMENT config * (EFFECTIVE_BALANCE_INCREMENT config * BASE_REWARD_FACTOR config div sqrt' (total_active_balance_f pbc)))" for f])
+    apply (erule get_base_reward_fast_wp)
+    apply (intro conjI impI; clarsimp?)
+  apply (fastforce)
+   apply (erule hoare_eqI')
+  apply (clarsimp)
+  apply (erule sep_conj_impl, assumption)
+  apply (sep_cancel)+
+  apply (sep_mp)
+  apply (subgoal_tac "list.set (local.range 0 (unat (MAX_EFFECTIVE_BALANCE + EFFECTIVE_BALANCE_INCREMENT config)) (unat (EFFECTIVE_BALANCE_INCREMENT config))) \<noteq> {}")
+   apply (clarsimp simp: nonempty_ball_conj_lift nonempty_ball_imp_lift)
+   apply (erule_tac x=0 in ballE; clarsimp?)
+  apply (clarsimp simp: range_empty_iff)
+  by (metis (mono_tags, opaque_lifting) add_0
+           ebi_not_zero effective_balance_safe gr0I unat_eq_zero word_coorder.extremum_uniqueI)
+  
+
+lemma read_beacon_wp_alt[wp]: "(\<And>x. hoare_triple ( lift (P x)) (c x) (Q )) \<Longrightarrow>
+   hoare_triple (lift (maps_to l v \<and>* (maps_to l v \<longrightarrow>* (\<lambda>s. x = v \<and> (x = v \<longrightarrow> (P v s)))))) 
+  (do {v <- read_beacon l ; c v}) (Q  )"
+  apply (clarsimp simp: hoare_triple_def bindCont_def run_def read_beacon_def getState_def )
+  apply (clarsimp simp: Sup_le_iff)
+  apply (safe)
+   apply (clarsimp simp: fail_def assert_galois_test)
+   defer
+   apply (clarsimp simp: fail_def assert_galois_test return_def)
+   apply (case_tac "y = v"; clarsimp?)
+    apply (subst seq_assoc[symmetric])
+    apply (subst test_seq_test)
+    apply (rule order_trans, rule seq_mono_left)
+     apply (rule test.hom_mono[where p="Collect (lift (P v))"])
+     apply (clarsimp)
+  apply (sep_select_asm 2)
+     apply (frule sep_mp)
+  apply (clarsimp)
+  apply (sep_mp, clarsimp)
+     apply (erule lift_mono, clarsimp, sep_solve)
+    apply (blast)
+  apply (subst seq_assoc[symmetric])
+   apply (subst test_seq_test)
+ apply (rule order_trans, rule seq_mono_left)
+    apply (rule test.hom_mono[where p="{}"])
+    apply (clarsimp)
+    defer
+    apply (clarsimp)
+  apply (subst seq_assoc[symmetric])
+   apply (subst test_seq_test)
+ apply (rule order_trans, rule seq_mono_left)
+    apply (rule test.hom_mono[where p="{}"])
+    apply (clarsimp)
+    defer
+     apply (clarsimp)
+  sorry
+   apply (drule maps_to_get_wf, clarsimp)
+  apply (drule maps_to_get_wf, clarsimp)
+  done
+
+abbreviation "map_var f vs \<equiv> map f (var_list_inner vs)"
+
+text \<open>[where x=x and v="\<lparr> effective_balances_f = (map_var Validator.effective_balance_f vs), 
+      base_rewards_f = (map (\<lambda>effective_balance.
+                             word_of_nat effective_balance div EFFECTIVE_BALANCE_INCREMENT config * (EFFECTIVE_BALANCE_INCREMENT config * BASE_REWARD_FACTOR config div sqrt' (total_active_balance_f pbc)))
+                      (local.range 0 (unat (MAX_EFFECTIVE_BALANCE + EFFECTIVE_BALANCE_INCREMENT config)) (unat (EFFECTIVE_BALANCE_INCREMENT config)))) \<rparr>"\<close>
+
+
+thm hoare_assert_stateI
+
+lemma hoare_eqI''': "hoare_triple (lift (P x)) (f x) Q \<Longrightarrow> v = x \<Longrightarrow>  hoare_triple (lift (P v)) (f v) Q"
+  apply (rule hoare_assert_stateI)
+  apply (clarsimp)
+  apply (clarsimp simp: lift_def)
+  apply (erule hoare_weaken_pre)
+  apply (clarsimp simp: lift_def)
+  apply (blast)
+  done
+
+lemma hoare_eqI_weaken: "hoare_triple (lift (P x)) (f x) Q \<Longrightarrow> (\<And>s. P' v s \<Longrightarrow> P x s) \<Longrightarrow> hoare_triple (lift (\<lambda>s. x = v \<and> (x = v \<longrightarrow> P' v s))) (f v) Q"
+  apply (rule hoare_assert_stateI)
+  apply (clarsimp)
+  apply (clarsimp simp: lift_def)
+  apply (erule hoare_weaken_pre)
+  apply (clarsimp simp: lift_def)
+  apply (blast)
+  done
+
+lemma read_beacon_wp'[wp]: "(\<And>x. hoare_triple ( lift (P x)) (c x) (Q )) \<Longrightarrow> 
+hoare_triple (lift (maps_to l v \<and>* (maps_to l v \<longrightarrow>*  (P v )))) (do {v <- read_beacon l ; c v}) (Q  )"
+  apply (wp)
+  done
+
+definition "base_rewards_from_cache pbc \<equiv>
+map (\<lambda>effective_balance. word_of_nat effective_balance div EFFECTIVE_BALANCE_INCREMENT config *
+      (EFFECTIVE_BALANCE_INCREMENT config * BASE_REWARD_FACTOR config div sqrt' (total_active_balance_f pbc)))
+       (local.range 0 (unat (MAX_EFFECTIVE_BALANCE + EFFECTIVE_BALANCE_INCREMENT config)) (unat (EFFECTIVE_BALANCE_INCREMENT config)))"
+
+schematic_goal new_base_rewards_cache_wp: 
+  "(\<And>x. hoare_triple (lift (P x)) (c x) Q) \<Longrightarrow> 
+hoare_triple (lift (validators \<mapsto>\<^sub>l vs \<and>* progressive_balances_cache \<mapsto>\<^sub>l pbc \<and>* 
+(validators \<mapsto>\<^sub>l vs \<and>* progressive_balances_cache \<mapsto>\<^sub>l pbc \<longrightarrow>*
+  (\<lambda>s. total_active_balance_f pbc < total_active_balance_f pbc + 1 \<and>
+       (total_active_balance_f pbc < total_active_balance_f pbc + 1 \<longrightarrow>
+        total_active_balance_f pbc \<noteq> 0 \<and>
+        (total_active_balance_f pbc \<noteq> 0 \<longrightarrow>
+         (\<forall>f\<in>list.set (local.range 0 (unat (MAX_EFFECTIVE_BALANCE + EFFECTIVE_BALANCE_INCREMENT config)) (unat (EFFECTIVE_BALANCE_INCREMENT config))).
+             safe_mul (word_of_nat f div EFFECTIVE_BALANCE_INCREMENT config) (EFFECTIVE_BALANCE_INCREMENT config * BASE_REWARD_FACTOR config div sqrt' (total_active_balance_f pbc)) \<and>
+             (safe_mul (word_of_nat f div EFFECTIVE_BALANCE_INCREMENT config) (EFFECTIVE_BALANCE_INCREMENT config * BASE_REWARD_FACTOR config div sqrt' (total_active_balance_f pbc)) \<longrightarrow>
+              P \<lparr>effective_balances_f = map_var Validator.effective_balance_f vs,
+                   base_rewards_f = base_rewards_from_cache pbc \<rparr> s)))))))) 
+       (bindCont new_base_rewards_cache c) Q"
+  apply (clarsimp simp: new_base_rewards_cache_def)
+  apply (rule hoare_weaken_pre, simp only: bindCont_assoc[symmetric])
+  apply (wp)
+
+   apply (clarsimp)
+  apply (sep_cancel)
+  apply (sep_cancel)+
+  apply (sep_mp)
+  apply (clarsimp)
+  apply (clarsimp simp: base_rewards_from_cache_def)
+  done
+
+
+lemma get_total_active_balance_wp[wp]:"(\<And>x. hoare_triple (lift (P x)) (c x) Q) \<Longrightarrow> 
+ hoare_triple (lift (beacon_slots \<mapsto>\<^sub>l b_s \<and>* validators \<mapsto>\<^sub>l vs \<and>*
+ (beacon_slots \<mapsto>\<^sub>l b_s \<and>* validators \<mapsto>\<^sub>l vs \<longrightarrow>* 
+(\<lambda>s. (\<forall>x\<in>list.set (active_validator_indices (slot_to_epoch config b_s) vs). x < var_list_len vs) \<and>
+       ((\<forall>x\<in>list.set (active_validator_indices (slot_to_epoch config b_s) vs). x < var_list_len vs) \<longrightarrow>
+        (\<forall>xs\<in>lists_of (list.set (active_validator_indices (slot_to_epoch config b_s) vs)).
+  P (max (EFFECTIVE_BALANCE_INCREMENT config)
+     (\<Sum>a\<leftarrow>xs. Validator.effective_balance_f (unsafe_var_list_index vs a))) s)  )))))
+ (bindCont get_total_active_balance c) Q"
+  apply (clarsimp simp: get_total_active_balance_def, rule hoare_weaken_pre, wp, clarsimp)
+  apply (sep_cancel)+
+  apply (sep_mp, clarsimp)
+  done
+
+find_theorems get_unslashed_participating_indices
+
+thm get_current_unslashed_participating_indices_wp
+
+
+abbreviation "current_epoch bs \<equiv> slot_to_epoch config bs"
+
+definition "unslashed_participating_indices flag_index epoch epoch_participation vs  \<equiv>
+            {x \<in> list.set (active_validator_indices epoch vs). 
+             has_flag (unsafe_var_list_index epoch_participation x) flag_index \<and> 
+             \<not> slashed_f (unsafe_var_list_index vs x)} 
+            "
+
+lemma get_flag_attesting_balance_current_epoch_wp: 
+  "(\<And>x. hoare_triple (lift (P x)) (c x) Q) \<Longrightarrow>
+   hoare_triple (lift (beacon_slots \<mapsto>\<^sub>l b_s \<and>* current_epoch_participation \<mapsto>\<^sub>l cep \<and>* 
+                       validators \<mapsto>\<^sub>l vs \<and>*
+                       (beacon_slots \<mapsto>\<^sub>l b_s \<and>* current_epoch_participation \<mapsto>\<^sub>l cep \<and>* 
+                         validators \<mapsto>\<^sub>l vs \<longrightarrow>*
+                         (\<lambda>s. epoch = current_epoch b_s \<and>
+                       (\<forall>x\<in>(unslashed_participating_indices flag_index epoch cep vs ). x < var_list_len vs) \<and>
+                        (epoch = current_epoch b_s \<longrightarrow>
+                        (\<forall>x\<in>(unslashed_participating_indices flag_index epoch cep vs ). x < var_list_len vs) \<longrightarrow> 
+        (\<forall>xs\<in>lists_of (unslashed_participating_indices flag_index epoch cep vs).
+         P (max (EFFECTIVE_BALANCE_INCREMENT config) (\<Sum>a\<leftarrow>xs. Validator.effective_balance_f (unsafe_var_list_index vs a))) s))))))
+      (bindCont (get_flag_attesting_balance flag_index epoch) c) Q"
+  apply (clarsimp simp: get_flag_attesting_balance_def, rule hoare_weaken_pre)
+  apply (clarsimp simp: bindCont_assoc[symmetric])
+   apply (rule hoare_eqI'[where v=epoch], rule get_current_unslashed_participating_indices_wp, wp)
+  apply (rule lift_mono')
+  apply (clarsimp)
+  apply (intro conjI)
+   apply (sep_mp)
+   apply (blast)
+  apply (clarsimp)
+  apply (sep_cancel)+
+  apply (sep_mp)
+  apply (clarsimp simp: unslashed_participating_indices_def)
+  done
+
+lemma get_flag_attesting_balance_previous_epoch_wp: 
+  "(\<And>x. hoare_triple (lift (P x)) (c x) Q) \<Longrightarrow> current_epoch b_s \<noteq> GENESIS_EPOCH \<Longrightarrow>
+   hoare_triple (lift (beacon_slots \<mapsto>\<^sub>l b_s \<and>* previous_epoch_participation \<mapsto>\<^sub>l pep \<and>* current_epoch_participation \<mapsto>\<^sub>l cep \<and>*
+                       validators \<mapsto>\<^sub>l vs \<and>*
+                       (beacon_slots \<mapsto>\<^sub>l b_s \<and>* previous_epoch_participation \<mapsto>\<^sub>l pep \<and>* current_epoch_participation \<mapsto>\<^sub>l cep \<and>* 
+                         validators \<mapsto>\<^sub>l vs \<longrightarrow>*
+                         (\<lambda>s. epoch = previous_epoch (slot_to_epoch config b_s) \<and>
+                       (\<forall>x\<in>(unslashed_participating_indices flag_index epoch pep vs). x < var_list_len vs) \<and>
+                        (epoch = previous_epoch (slot_to_epoch config b_s) \<longrightarrow>
+                        (\<forall>x\<in>(unslashed_participating_indices flag_index epoch pep vs). x < var_list_len vs) \<longrightarrow> 
+        (\<forall>xs\<in>lists_of (unslashed_participating_indices flag_index epoch pep vs).
+         P (max (EFFECTIVE_BALANCE_INCREMENT config) (\<Sum>a\<leftarrow>xs. Validator.effective_balance_f (unsafe_var_list_index vs a))) s))))))
+      (bindCont (get_flag_attesting_balance flag_index epoch) c) Q"
+  apply (clarsimp simp: get_flag_attesting_balance_def, rule hoare_weaken_pre)
+  apply (clarsimp simp: bindCont_assoc[symmetric])
+   apply (rule hoare_eqI'[where v=epoch], rule get_previous_unslashed_participating_indices_wp, wp)
+  apply (rule lift_mono')
+  apply (clarsimp)
+  apply (intro conjI)
+   apply (sep_mp)
+   apply (blast)
+  apply (clarsimp)
+  apply (sep_cancel)+
+  apply (sep_mp)
+  apply (clarsimp simp: unslashed_participating_indices_def)
+  done
+
+
+lemma val_length_wf:  "(validators \<mapsto>\<^sub>l vs \<and>* R) s \<Longrightarrow> length (local.var_list_inner vs) \<le> 2 ^ 64 - 1"
+  sorry
+
+lemma new_progressive_balances_wp: "(\<And>x. hoare_triple (lift (P x)) (c x) Q) \<Longrightarrow>
+  hoare_triple (lift (beacon_slots \<mapsto>\<^sub>l b_s \<and>* validators \<mapsto>\<^sub>l vs \<and>*
+                     current_epoch_participation \<mapsto>\<^sub>l cep \<and>*
+                     previous_epoch_participation \<mapsto>\<^sub>l pep \<and>* 
+                    (beacon_slots \<mapsto>\<^sub>l b_s \<and>* validators \<mapsto>\<^sub>l vs \<and>*
+                     current_epoch_participation \<mapsto>\<^sub>l cep \<and>*
+                     previous_epoch_participation \<mapsto>\<^sub>l pep  \<longrightarrow>*
+ (\<lambda>s.(\<exists>ep. ep = (if (current_epoch b_s) = GENESIS_EPOCH then cep else pep) \<and>  
+     (\<forall>xs \<in> lists_of (list.set (active_validator_indices (current_epoch b_s) vs)).
+     \<forall>xsa \<in> lists_of (unslashed_participating_indices TIMELY_SOURCE_FLAG_INDEX (previous_epoch (current_epoch b_s)) ep vs).
+     \<forall>xsb \<in> lists_of (unslashed_participating_indices TIMELY_TARGET_FLAG_INDEX (previous_epoch (current_epoch b_s)) ep vs).
+     \<forall>xsc \<in> lists_of (unslashed_participating_indices TIMELY_HEAD_FLAG_INDEX   (previous_epoch (current_epoch b_s)) ep vs).
+     \<forall>xsd \<in> lists_of (unslashed_participating_indices TIMELY_SOURCE_FLAG_INDEX (current_epoch b_s) cep vs).
+     \<forall>xse \<in> lists_of (unslashed_participating_indices TIMELY_TARGET_FLAG_INDEX (current_epoch b_s) cep vs).
+     \<forall>xsf \<in> lists_of (unslashed_participating_indices TIMELY_HEAD_FLAG_INDEX (current_epoch b_s) cep vs).
+      P (ProgressiveBalancesCache.fields (max (EFFECTIVE_BALANCE_INCREMENT config) (\<Sum>a\<leftarrow>xs. Validator.effective_balance_f (unsafe_var_list_index vs a)))
+           [max (EFFECTIVE_BALANCE_INCREMENT config) (\<Sum>a\<leftarrow>xsa. Validator.effective_balance_f (unsafe_var_list_index vs a)),
+            max (EFFECTIVE_BALANCE_INCREMENT config) (\<Sum>a\<leftarrow>xsb. Validator.effective_balance_f (unsafe_var_list_index vs a)),
+            max (EFFECTIVE_BALANCE_INCREMENT config) (\<Sum>a\<leftarrow>xsc. Validator.effective_balance_f (unsafe_var_list_index vs a))]
+           [max (EFFECTIVE_BALANCE_INCREMENT config) (\<Sum>a\<leftarrow>xsd. Validator.effective_balance_f (unsafe_var_list_index vs a)),
+            max (EFFECTIVE_BALANCE_INCREMENT config) (\<Sum>a\<leftarrow>xse. Validator.effective_balance_f (unsafe_var_list_index vs a)),
+            max (EFFECTIVE_BALANCE_INCREMENT config) (\<Sum>a\<leftarrow>xsf. Validator.effective_balance_f (unsafe_var_list_index vs a))]) s))))))
+ (bindCont new_progressive_balances c) Q"
+  apply (case_tac "current_epoch b_s = GENESIS_EPOCH")
+defer
+  apply (clarsimp simp: new_progressive_balances_def, rule hoare_weaken_pre)
+  apply (clarsimp simp: bindCont_assoc[symmetric])
+   apply (rule get_total_active_balance_wp[where b_s=b_s])
+   apply (rule get_previous_epoch_wp[where v=b_s])
+   apply (rule get_current_epoch_wp[where v=b_s])
+   apply (rule get_flag_attesting_balance_previous_epoch_wp[where b_s=b_s])
+   apply (rule get_flag_attesting_balance_previous_epoch_wp[where b_s=b_s])
+   apply (rule get_flag_attesting_balance_previous_epoch_wp[where b_s=b_s])
+   apply (rule get_flag_attesting_balance_current_epoch_wp[where b_s=b_s])+
+   apply (fastforce)
+     apply (clarsimp)
+     prefer 3
+  apply (clarsimp)
+  apply (sep_cancel)+
+  apply (safe; clarsimp?)
+  apply (erule active_validator_indices_are_bound)
+   apply (clarsimp simp: sep_conj_assoc)
+   apply (sep_drule (direct) val_length_wf)
+   apply (clarsimp)
+  apply (clarsimp simp: sep_conj_assoc)
+  apply (sep_cancel)+
+     apply (intro conjI)
+      apply (clarsimp simp: unslashed_participating_indices_def)
+ apply (erule active_validator_indices_are_bound)
+   apply (clarsimp simp: sep_conj_assoc)
+   apply (sep_drule (direct) val_length_wf)
+      apply (clarsimp)
+     apply (intro conjI impI ballI)
+     apply (sep_cancel)+
+     apply (intro conjI impI ballI)
+      apply (clarsimp simp: unslashed_participating_indices_def)
+
+apply (erule active_validator_indices_are_bound)
+   apply (clarsimp simp: sep_conj_assoc)
+   apply (sep_drule (direct) val_length_wf)
+      apply (clarsimp)
+     apply (sep_cancel)+
+ apply (intro conjI impI ballI)
+      apply (clarsimp simp: unslashed_participating_indices_def)
+
+apply (erule active_validator_indices_are_bound)
+   apply (clarsimp simp: sep_conj_assoc)
+   apply (sep_drule (direct) val_length_wf)
+      apply (clarsimp)
+     apply (sep_cancel)+
+ apply (intro conjI impI ballI)
+      apply (clarsimp simp: unslashed_participating_indices_def)
+
+     apply (sep_cancel)+
+  apply (intro conjI impI)
+      apply (clarsimp simp: unslashed_participating_indices_def)
+     apply (intro conjI impI ballI)
+     apply (sep_cancel)+
+     apply (intro conjI impI ballI)
+      apply (clarsimp simp: unslashed_participating_indices_def)
+   apply (clarsimp simp: sep_conj_assoc)
+     apply (sep_mp)
+  apply (erule_tac x=xs in ballE)
+      apply (erule_tac x=xsa in ballE)
+       apply (erule_tac x=xsb in ballE)
+        apply (erule_tac x=xsc in ballE)
+         apply (erule_tac x=xsd in ballE)
+          apply (erule_tac x=xse in ballE)
+  apply (erule_tac x=xsf in ballE)
+            apply (assumption)
+           apply (clarsimp)+
+  apply (clarsimp simp: new_progressive_balances_def, rule hoare_weaken_pre)
+   apply (clarsimp simp: bindCont_assoc[symmetric])
+apply (rule get_total_active_balance_wp[where b_s=b_s])
+   apply (rule get_previous_epoch_wp[where v=b_s])
+  apply (rule get_current_epoch_wp[where v=b_s])
+   apply (rule get_flag_attesting_balance_current_epoch_wp[where b_s=b_s])+
+   apply (fastforce)
+apply (clarsimp)
+  apply (sep_cancel)+
+  apply (safe; clarsimp?)
+  apply (erule active_validator_indices_are_bound)
+   apply (clarsimp simp: sep_conj_assoc)
+   apply (sep_drule (direct) val_length_wf)
+   apply (clarsimp)
+  apply (clarsimp simp: sep_conj_assoc)
+  apply (sep_cancel)+
+     apply (intro conjI impI ballI)
+   apply (clarsimp simp: unslashed_participating_indices_def)
+  apply (sep_cancel)+
+
+  apply (intro conjI impI ballI)
+   apply (clarsimp simp: unslashed_participating_indices_def)
+  apply (sep_cancel)+
+  apply (intro conjI impI ballI)
+   apply (clarsimp simp: unslashed_participating_indices_def)
+  apply (sep_cancel)+
+  apply (intro conjI impI ballI)
+   apply (clarsimp simp: unslashed_participating_indices_def)
+  apply (sep_cancel)+
+ apply (intro conjI impI ballI)
+   apply (clarsimp simp: unslashed_participating_indices_def)
+apply (sep_cancel)+
+ apply (intro conjI impI ballI)
+   apply (clarsimp simp: unslashed_participating_indices_def)
+  apply (clarsimp simp: sep_conj_assoc)
+  apply (sep_mp)
+  apply (clarsimp)
+  done  
+
+lemma mapM_wp_foldr':
+  assumes c_wp: "\<And>(f :: 'e \<Rightarrow> ('f, 'a) cont) x P Q. (\<And>x. hoare_triple (lift (P x)) (f x) (Q)) \<Longrightarrow> 
+                                                    hoare_triple (lift (pre (P (g x)) x)) (do { b <- c x; f b}) Q"  
+  shows " (\<And>x. hoare_triple (lift (P x)) (f x) Q) 
+          \<Longrightarrow>   hoare_triple (lift (foldr (\<lambda>x R. pre R x) xs (P (map g xs)) ))
+                (do {vs <- mapM c (xs :: 'd list) ; (f :: 'e list \<Rightarrow> ('f, 'a) cont) (vs )}) Q"
+  apply (induct xs arbitrary: P f; clarsimp)
+  apply (rule hoare_weaken_pre, subst bindCont_assoc[symmetric])
+   apply (rule c_wp)
+   apply (atomize, erule allE)
+  apply (erule allE) back
+  apply (subst bindCont_assoc[symmetric])
+   apply (erule mp)
+   apply (clarsimp)
+   apply (fastforce)
+  apply (fastforce)
+  done
+
+lemma sep_factor_foldI':
+  "(I \<and>* (foldr (\<lambda>x R. (P x \<and>* (Q x \<longrightarrow>* R))) xs (I \<longrightarrow>* R))) s \<Longrightarrow> (foldr (\<lambda>x R. (I \<and>* P x \<and>* (I \<and>* Q x \<longrightarrow>* R))) xs R) s"
+  apply (induct xs arbitrary:s; clarsimp simp:)
+   apply (sep_solve)
+  apply (sep_cancel)+
+  apply (sep_mp)
+  apply (clarsimp simp: sep_conj_ac)
+  done
+
+lemma factor_foldr_conj: "(\<forall>x\<in>(list.set xs). P x) \<and> (foldr f xs R) s \<Longrightarrow> (\<And>a. mono (f a)) \<Longrightarrow>  
+  (foldr (\<lambda>x R s. P x \<and> f x R s) xs R) s"
+  apply (induct xs  arbitrary: s; clarsimp)
+  by (metis (mono_tags, lifting) monoD predicate1D predicate1I)
+
+
+lemma factor_foldr_pure: "(\<forall>x\<in>(list.set xs). P x) \<and> ((\<forall>x\<in>(list.set xs). P x) \<longrightarrow> (foldr f xs R) s) \<Longrightarrow> (\<And>a. mono (f a)) \<Longrightarrow>  
+  (foldr (\<lambda>x R s. (P x \<longrightarrow> f x R s) \<and> P x) xs R) s"
+  apply (induct xs  arbitrary: s; clarsimp)
+  apply (atomize)
+  by (metis (mono_tags, lifting) le_boolD le_funE monoD predicate1I)
+
+lemma factor_foldr_conj': "(\<forall>x\<in>(list.set xs). P x) \<and> (foldr f xs R) s \<Longrightarrow> (\<And>a. mono (f a)) \<Longrightarrow>  
+  (foldr (\<lambda>x R s. f x R s \<and> P x) xs R) s"
+  apply (induct xs  arbitrary: s; clarsimp)
+  by (metis (mono_tags, lifting) monoD predicate1D predicate1I)
+
+
+lemma factor_foldr_sep: "(P \<and>* (foldr f xs (P \<longrightarrow>* R))) s \<Longrightarrow> (\<And>a. mono (f a)) \<Longrightarrow>  (\<And>R a. f a (P \<and>* R) = (P \<and>* f a R)) \<Longrightarrow>   (foldr (\<lambda>x R. P \<and>* (P \<longrightarrow>* f x R)) xs  R) s"
+  apply (induct xs  arbitrary: s; clarsimp)
+   apply (sep_mp, clarsimp)
+  apply (sep_cancel)+
+  apply (erule sep_curry[rotated])
+  apply (clarsimp simp: sep_conj_ac)
+  by (smt (verit, ccfv_threshold) monoE predicate1D predicate1I sep_conj_commute)
+  apply (erule_tac x=h in allE)
+  apply (drule mp)
+   apply (sep_cancel)
+  oops
+
+lemma in_set_pure_simp[simp]:"in_set (\<lambda>_. P) s = P"
+  by (clarsimp simp: in_set_def)
+
+declare range.simps[simp del ]
+
+lemma foldr_const[simp]: "foldr (\<lambda>_ R. R) xs R = R"
+  by (induct xs; clarsimp)
+
+
+lemma mono_id[simp]: "mono (\<lambda>R. R)" 
+   by (rule monoI; clarsimp)
+
+
+lemma new_rewards_and_penalties_context_wp[wp]:"(\<And>x. hoare_triple (lift (P x)) (c x) Q) \<Longrightarrow>
+   hoare_triple 
+          (lift (progressive_balances_cache \<mapsto>\<^sub>l pbc \<and>* 
+          (\<lambda>s. (\<forall>x\<in>list.set (local.range 0 (unat NUM_FLAG_INDICES) (Suc 0)). x < length (previous_epoch_flag_attesting_balances_f pbc)) \<and>
+         ((\<forall>x\<in>list.set (local.range 0 (unat NUM_FLAG_INDICES) (Suc 0)). x < length (previous_epoch_flag_attesting_balances_f pbc)) \<longrightarrow>
+          (progressive_balances_cache \<mapsto>\<^sub>l pbc \<longrightarrow>*
+           P (RewardsAndPenaltiesContext.fields (map (\<lambda>a. previous_epoch_flag_attesting_balances_f pbc ! a div EFFECTIVE_BALANCE_INCREMENT config) (local.range 0 (unat NUM_FLAG_INDICES) (Suc 0)))
+               (total_active_balance_f pbc div EFFECTIVE_BALANCE_INCREMENT config)))s
+           )))) 
+   (bindCont (new_rewards_and_penalties_context pbc) c) Q"
+  apply (unfold new_rewards_and_penalties_context_def)
+  apply (rule hoare_weaken_pre)
+   apply (simp only: bindCont_assoc[symmetric])
+   apply (rule mapM_wp_foldr')
+    apply (clarsimp simp: unslashed_participating_increment_def liftM_def comp_def)
+   apply (simp only: bindCont_assoc[symmetric])
+  apply (rule read_beacon_wp[where v=pbc])
+    apply (wp)
+    apply (clarsimp)
+   apply (wp)
+  apply (rule lift_mono')
+  apply (safe)
+  apply (simp only: in_set_pure_simp[simp] ebi_not_zero)
+  apply (clarsimp)
+  apply (rule factor_foldr_sep)
+    prefer 2
+    apply (clarsimp simp: mono_def)
+    apply blast
+   defer
+   apply (intro ext iffI; clarsimp)
+  apply (sep_cancel)
+  apply (rule factor_foldr_pure)
+   apply (clarsimp)
+  by (clarsimp)
+
+find_theorems new_effective_balances_ctxt
+
+lemma EBI_multiple_of_HYSTERESIS_QUOTIENT: 
+  "\<exists>n. HYSTERESIS_QUOTIENT * n div n = HYSTERESIS_QUOTIENT \<and> EFFECTIVE_BALANCE_INCREMENT config = HYSTERESIS_QUOTIENT * n" sorry
+
+lemma upward_threshold_safe: "((EFFECTIVE_BALANCE_INCREMENT config div HYSTERESIS_QUOTIENT) * HYSTERESIS_UPWARD_MULTIPLIER)
+         div (EFFECTIVE_BALANCE_INCREMENT config div HYSTERESIS_QUOTIENT) = HYSTERESIS_UPWARD_MULTIPLIER"
+  sorry
+
+lemma safe_mul_one[simp]: "safe_mul 1 (x :: u64)"
+  apply (clarsimp simp: safe_mul_def)
+  using div_word_self by blast
+
+lemma new_effective_balances_ctxt_wp[wp]: 
+"(\<And>x. hoare_triple (lift (P x)) (c x) Q) \<Longrightarrow>
+  hoare_triple 
+    (lift (P \<lparr> downward_threshold_f = 
+                (EFFECTIVE_BALANCE_INCREMENT config div HYSTERESIS_QUOTIENT), 
+              upward_threshold_f = 
+                (EFFECTIVE_BALANCE_INCREMENT config div HYSTERESIS_QUOTIENT * HYSTERESIS_UPWARD_MULTIPLIER)\<rparr>)) 
+     (bindCont new_effective_balances_ctxt c) Q "
+  apply (unfold new_effective_balances_ctxt_def, rule hoare_weaken_pre, wp)
+  apply (clarsimp simp: HYSTERESIS_QUOTIENT_def HYSTERESIS_DOWNWARD_MULTIPLIER_def HYSTERESIS_UPWARD_MULTIPLIER_def)
+  apply (intro conjI impI)
+  using EBI_multiple_of_HYSTERESIS_QUOTIENT 
+    apply (insert EBI_multiple_of_HYSTERESIS_QUOTIENT)[1]
+   apply (clarsimp simp: HYSTERESIS_QUOTIENT_def)
+   apply (clarsimp simp: safe_mul_def)
+  apply (metis HYSTERESIS_QUOTIENT_def HYSTERESIS_UPWARD_MULTIPLIER_def mult.commute upward_threshold_safe)
+  by (clarsimp simp: EffectiveBalancesContext.defs)
+
+
+
+lemma new_next_epoch_progressive_balances_wp[wp]: "(\<And>x. hoare_triple (lift (P x)) (c x) Q) \<Longrightarrow>
+  hoare_triple 
+    (lift (\<lambda>s. P \<lparr> total_active_balance_f = 0, 
+                   previous_epoch_flag_attesting_balances_f = current_epoch_flag_attesting_balances_f pbc,
+                   current_epoch_flag_attesting_balances_f = [0,0,0]\<rparr> s)) 
+   (bindCont (new_next_epoch_progressive_balances pbc) c) Q"
+  by (clarsimp simp: new_next_epoch_progressive_balances_def ProgressiveBalancesCache.defs)
+
+term "effective_balances_f brc ! unat n div EFFECTIVE_BALANCE_INCREMENT config = (effective_balances_f brc ! unat n) div EFFECTIVE_BALANCE_INCREMENT config"
+
+lemma get_cached_base_reward_wp[wp]:"(\<And>x. hoare_triple (lift (P x)) (c x) Q) \<Longrightarrow>
+  hoare_triple 
+   (lift (\<lambda>s. (length (base_rewards_f brc) \<le> 2 ^ 64 - 1) \<and> n < word_of_nat (length (effective_balances_f brc)) \<and>  effective_balances_f brc ! unat n div EFFECTIVE_BALANCE_INCREMENT config < word_of_nat (length (base_rewards_f brc))
+              \<and>  (n < word_of_nat (length (effective_balances_f brc)) \<longrightarrow> effective_balances_f brc ! unat n div EFFECTIVE_BALANCE_INCREMENT config < word_of_nat (length (base_rewards_f brc)) \<longrightarrow> length (base_rewards_f brc) \<le> 2 ^ 64 - 1 \<longrightarrow>
+    (P (base_rewards_f brc ! unat (effective_balances_f brc ! unat n div EFFECTIVE_BALANCE_INCREMENT config)) s))))
+   (bindCont (get_cached_base_reward brc n) c)
+    Q"
+  apply (clarsimp simp: get_cached_base_reward_def, rule hoare_weaken_pre, wp)
+  apply (clarsimp)
+  by (simp add: ebi_not_zero)
+
+
+definition single_inactivity_update:: "u64 \<Rightarrow> ValidatorInfo \<Rightarrow> StateContext \<Rightarrow> u64"
+  where "single_inactivity_update inactivity_score val_info state_ctxt \<equiv> 
+  if \<not>(is_eligible_f val_info) then inactivity_score
+  else 
+  (let new_inactivity_score = inactivity_score in
+   let new_inactivity_score = (if (is_unslashed_participating_index val_info TIMELY_TARGET_FLAG_INDEX)
+                              then (new_inactivity_score - (min new_inactivity_score 1))
+                              else (new_inactivity_score + INACTIVITY_SCORE_BIAS config)) in
+   let new_inactivity_score = (if \<not>(is_in_inactivity_leak_f state_ctxt)
+                              then (new_inactivity_score - (min new_inactivity_score (INACTIVITY_SCORE_RECOVERY_RATE config)))
+                              else (new_inactivity_score))
+  in new_inactivity_score)
+"
+
+lemma process_single_inactivity_update_wp[wp]: "(\<And>x. hoare_triple (lift (P x)) (c x) Q) \<Longrightarrow>
+  hoare_triple (lift (\<lambda>s. inactivity_score \<le> inactivity_score + INACTIVITY_SCORE_BIAS config \<and>
+                          (inactivity_score \<le> inactivity_score + INACTIVITY_SCORE_BIAS config \<longrightarrow> 
+                             P (single_inactivity_update inactivity_score validator_info state_ctxt) s )))
+   (bindCont (process_single_inactivity_update inactivity_score validator_info state_ctxt) c)
+   Q"
+  apply (unfold process_single_inactivity_update_def, rule hoare_weaken_pre, wp)
+    apply (clarsimp)
+  apply (fastforce)
+   apply (simp only: Let_unfold)
+   apply (wp)
+    apply (clarsimp, wp)
+   apply (clarsimp ,wp)
+  apply (clarsimp)
+  apply (safe)
+         apply (clarsimp simp: single_inactivity_update_def Let_unfold)+
+  done
+
+
+lemma hoare_let[intro, wp]: "hoare_triple P (bindCont (b a) c) Q \<Longrightarrow> hoare_triple P (bindCont (Let a b) c) Q"
+  by (clarsimp simp: Let_unfold)
+
+
+definition "rewardable (v_info :: ValidatorInfo) flag_index state_ctxt \<equiv> 
+              (is_unslashed_participating_index v_info flag_index) \<and>
+              \<not>(is_in_inactivity_leak_f state_ctxt)"
+
+
+
+
+lemma if_lift: "(if B then lift P else lift Q) = lift (if B then P else Q)"
+  by (intro ext; clarsimp simp: lift_def)
+
+thm mul_wp
+
+lemma get_flag_index_delta_TIMELY_SOURCE_WEIGHT_wp[wp]: "(\<And>x. hoare_triple (lift (P x)) (c x) Q) \<Longrightarrow>
+   hoare_triple (lift (\<lambda>s. let unslashed_participating_increment = (unslashed_participating_increments_array_f rewards_ctxt ! 0) in
+                            safe_mul TIMELY_SOURCE_WEIGHT (base_reward_f v_info) \<and> 
+                            safe_mul (TIMELY_SOURCE_WEIGHT * base_reward_f v_info) unslashed_participating_increment \<and>
+                            safe_mul (active_increments_f rewards_ctxt) WEIGHT_DENOMINATOR \<and> 
+                            active_increments_f rewards_ctxt * WEIGHT_DENOMINATOR \<noteq> 0 \<and> 
+                           (safe_mul TIMELY_SOURCE_WEIGHT (base_reward_f v_info) \<and> 
+                            safe_mul (TIMELY_SOURCE_WEIGHT * base_reward_f v_info) unslashed_participating_increment \<and>
+                            safe_mul (active_increments_f rewards_ctxt) WEIGHT_DENOMINATOR \<and> 
+                            active_increments_f rewards_ctxt * WEIGHT_DENOMINATOR \<noteq> 0 \<longrightarrow> 
+              (if rewardable v_info 0 state_ctxt then 
+                 P (base_reward_f v_info * TIMELY_SOURCE_WEIGHT * unslashed_participating_increment div (active_increments_f rewards_ctxt * WEIGHT_DENOMINATOR), 0) s
+            else P (0, base_reward_f v_info * TIMELY_SOURCE_WEIGHT div WEIGHT_DENOMINATOR) s)) )) 
+                (bindCont (get_flag_index_delta v_info 0 rewards_ctxt state_ctxt) c) Q"
+  apply (clarsimp simp: get_flag_index_delta_def, rule hoare_weaken_pre)
+   apply (wp)
+   apply (clarsimp simp: , assumption)
+  apply (subst if_lift)+
+  apply (rule lift_mono')
+  apply (simp add: TIMELY_HEAD_FLAG_INDEX_def PARTICIPATION_FLAG_WEIGHTS_def) 
+  apply (intro conjI impI; clarsimp simp: Let_unfold)
+   apply (clarsimp simp: rewardable_def)
+   apply (intro conjI impI)
+    apply (fastforce simp: safe_mul_commute mult.commute)
+  apply (fastforce simp: safe_mul_commute mult.commute)
+   apply (clarsimp simp: rewardable_def)
+  done
+
+lemma get_flag_index_delta_TIMELY_TARGET_WEIGHT_wp[wp]: "(\<And>x. hoare_triple (lift (P x)) (c x) Q) \<Longrightarrow>
+   hoare_triple (lift (\<lambda>s. let unslashed_participating_increment = (unslashed_participating_increments_array_f rewards_ctxt ! 1) in
+                            safe_mul TIMELY_TARGET_WEIGHT (base_reward_f v_info) \<and> 
+                            safe_mul (TIMELY_TARGET_WEIGHT * base_reward_f v_info) unslashed_participating_increment \<and>
+                            safe_mul (active_increments_f rewards_ctxt) WEIGHT_DENOMINATOR \<and> 
+                            active_increments_f rewards_ctxt * WEIGHT_DENOMINATOR \<noteq> 0 \<and> 
+                           (safe_mul TIMELY_TARGET_WEIGHT (base_reward_f v_info) \<and> 
+                            safe_mul (TIMELY_TARGET_WEIGHT * base_reward_f v_info) unslashed_participating_increment \<and>
+                            safe_mul (active_increments_f rewards_ctxt) WEIGHT_DENOMINATOR \<and> 
+                            active_increments_f rewards_ctxt * WEIGHT_DENOMINATOR \<noteq> 0 \<longrightarrow> 
+              (if rewardable v_info 1 state_ctxt then 
+                 P (base_reward_f v_info * TIMELY_TARGET_WEIGHT * unslashed_participating_increment div (active_increments_f rewards_ctxt * WEIGHT_DENOMINATOR), 0) s
+            else P (0, base_reward_f v_info * TIMELY_TARGET_WEIGHT div WEIGHT_DENOMINATOR) s)) )) 
+                (bindCont (get_flag_index_delta v_info 1 rewards_ctxt state_ctxt) c) Q"
+  apply (clarsimp simp: get_flag_index_delta_def, rule hoare_weaken_pre)
+   apply (wp)
+   apply (clarsimp simp: , assumption)
+  apply (subst if_lift)+
+  apply (rule lift_mono')
+  apply (simp add: TIMELY_HEAD_FLAG_INDEX_def PARTICIPATION_FLAG_WEIGHTS_def) 
+  apply (intro conjI impI; clarsimp simp: Let_unfold)
+   apply (clarsimp simp: rewardable_def)
+   apply (intro conjI impI)
+    apply (fastforce simp: safe_mul_commute mult.commute)
+  apply (fastforce simp: safe_mul_commute mult.commute)
+   apply (clarsimp simp: rewardable_def)
+  done
+
+thm get_flag_index_delta_def
+
+lemma get_flag_index_delta_wp_gen: "(\<And>x. hoare_triple (lift (P x)) (c x) Q) \<Longrightarrow>
+   hoare_triple (lift (\<lambda>s. let unslashed_participating_increment = (unslashed_participating_increments_array_f rewards_ctxt ! flag_index) in
+                           let weight = PARTICIPATION_FLAG_WEIGHTS ! flag_index in
+                            flag_index < length PARTICIPATION_FLAG_WEIGHTS \<and> 
+                            flag_index < length (unslashed_participating_increments_array_f rewards_ctxt) \<and>
+                            safe_mul weight (base_reward_f v_info) \<and> 
+                            safe_mul (weight * base_reward_f v_info) unslashed_participating_increment \<and>
+                            safe_mul (active_increments_f rewards_ctxt) WEIGHT_DENOMINATOR \<and> 
+                            active_increments_f rewards_ctxt * WEIGHT_DENOMINATOR \<noteq> 0 \<and> 
+                           (flag_index < length PARTICIPATION_FLAG_WEIGHTS \<and> 
+                            flag_index < length (unslashed_participating_increments_array_f rewards_ctxt) \<and>
+                            safe_mul weight (base_reward_f v_info) \<and> 
+                            safe_mul (weight * base_reward_f v_info) unslashed_participating_increment \<and>
+                            safe_mul (active_increments_f rewards_ctxt) WEIGHT_DENOMINATOR \<and> 
+                            active_increments_f rewards_ctxt * WEIGHT_DENOMINATOR \<noteq> 0 \<longrightarrow> 
+              (if rewardable v_info flag_index state_ctxt then 
+                 P (base_reward_f v_info * weight * unslashed_participating_increment div (active_increments_f rewards_ctxt * WEIGHT_DENOMINATOR), 0) s
+            else (if flag_index = TIMELY_HEAD_FLAG_INDEX then P (0, 0) s else P (0, base_reward_f v_info * weight div WEIGHT_DENOMINATOR) s))) )) 
+                (bindCont (get_flag_index_delta v_info flag_index rewards_ctxt state_ctxt) c) Q"
+  apply (clarsimp simp: get_flag_index_delta_def, rule hoare_weaken_pre)
+   apply (wp)
+   apply (clarsimp simp: , assumption)
+  apply (subst if_lift)+
+  apply (rule lift_mono')
+  apply (simp add: TIMELY_HEAD_FLAG_INDEX_def PARTICIPATION_FLAG_WEIGHTS_def) 
+  apply (intro conjI impI; clarsimp simp: Let_unfold)
+   apply (clarsimp simp: rewardable_def)
+   apply (intro conjI impI)
+    apply (fastforce simp: safe_mul_commute mult.commute)
+     apply (fastforce simp: safe_mul_commute mult.commute)
+    apply (clarsimp simp: rewardable_def)
+   apply (clarsimp simp: rewardable_def)
+   apply (fastforce simp: safe_mul_commute mult.commute)
+ apply (clarsimp simp: rewardable_def)
+  done
+
+lemma get_flag_index_delta_TIMELY_HEAD_WEIGHT_wp[wp]: "(\<And>x. hoare_triple (lift (P x)) (c x) Q) \<Longrightarrow>
+   hoare_triple (lift (\<lambda>s. let unslashed_participating_increment = (unslashed_participating_increments_array_f rewards_ctxt ! 2) in
+                            safe_mul TIMELY_HEAD_WEIGHT (base_reward_f v_info) \<and> 
+                            safe_mul (TIMELY_HEAD_WEIGHT * base_reward_f v_info) unslashed_participating_increment \<and>
+                            safe_mul (active_increments_f rewards_ctxt) WEIGHT_DENOMINATOR \<and> 
+                            active_increments_f rewards_ctxt * WEIGHT_DENOMINATOR \<noteq> 0 \<and> 
+                           (safe_mul TIMELY_HEAD_WEIGHT (base_reward_f v_info) \<and> 
+                            safe_mul (TIMELY_HEAD_WEIGHT * base_reward_f v_info) unslashed_participating_increment \<and>
+                            safe_mul (active_increments_f rewards_ctxt) WEIGHT_DENOMINATOR \<and> 
+                            active_increments_f rewards_ctxt * WEIGHT_DENOMINATOR \<noteq> 0 \<longrightarrow> 
+              (if rewardable v_info 2 state_ctxt then 
+                 P (base_reward_f v_info * TIMELY_HEAD_WEIGHT * unslashed_participating_increment div (active_increments_f rewards_ctxt * WEIGHT_DENOMINATOR), 0) s
+            else P (0, 0) s)) )) 
+                (bindCont (get_flag_index_delta v_info 2 rewards_ctxt state_ctxt) c) Q"
+  apply (clarsimp simp: get_flag_index_delta_def, rule hoare_weaken_pre)
+   apply (wp)
+   apply (clarsimp simp: , assumption)
+  apply (subst if_lift)+
+  apply (rule lift_mono')
+  apply (simp add: TIMELY_HEAD_FLAG_INDEX_def PARTICIPATION_FLAG_WEIGHTS_def) 
+  apply (intro conjI impI; clarsimp simp: Let_unfold)
+   apply (clarsimp simp: rewardable_def)
+   apply (intro conjI impI)
+    apply (fastforce simp: safe_mul_commute mult.commute)
+  apply (fastforce simp: safe_mul_commute mult.commute)
+   apply (clarsimp simp: rewardable_def)
+  done
+ 
+
+lemma range_participation_flag_weights_simp:"(local.range 0 (length PARTICIPATION_FLAG_WEIGHTS) 1) = [0,1,2]"
+  apply (clarsimp simp: PARTICIPATION_FLAG_WEIGHTS_def)
+  by (clarsimp simp: range.simps)
+
+term case_prod
+
+lemma hoare_case_prod[intro, wp]: "hoare_triple P (bindCont (f (fst x) (snd x)) c) Q \<Longrightarrow> 
+  hoare_triple P (bindCont (case_prod f x) c) Q"
+  by (clarsimp split: prod.splits)
+
+
+lemma add_wp'[wp]: "(\<And>x. hoare_triple (lift (P x )) (c x) Q) \<Longrightarrow>
+  hoare_triple (lift (\<lambda>s. n \<le> n + m \<and> (n \<le> n + m \<longrightarrow> P (n + m) s))) 
+(do {x <- (word_unsigned_add n  m); c x}) Q"
+  apply (rule hoare_weaken_pre)
+   apply (clarsimp simp:  word_unsigned_add_def )
+   apply (simp only: Let_unfold)
+   apply (wp, clarsimp simp: bindCont_return')
+    apply (fastforce)
+   apply (wp)
+  by (clarsimp)
+
+lemma ISB_not_zero[simp]:  "INACTIVITY_SCORE_BIAS config \<noteq> 0" sorry
+
+lemma safe_mul_not_zeroI:"safe_mul (x :: u64) y \<Longrightarrow> x \<noteq> 0 \<Longrightarrow> y \<noteq> 0 \<Longrightarrow> x * y \<noteq> 0"
+  by (clarsimp simp: safe_mul_def)
+
+lemma get_inactivity_penalty_delta_wp[wp]: "
+ (\<And>x. hoare_triple (lift (P x)) (c x) Q) \<Longrightarrow> 
+  hoare_triple (lift (\<lambda>s. let effective_balance = ValidatorInfo.effective_balance_f val_info in
+                          safe_mul inactivity_score effective_balance \<and>
+                          safe_mul INACTIVITY_PENALTY_QUOTIENT_ALTAIR (INACTIVITY_SCORE_BIAS config) \<and>
+                   (safe_mul inactivity_score effective_balance \<longrightarrow>
+                    safe_mul INACTIVITY_PENALTY_QUOTIENT_ALTAIR (INACTIVITY_SCORE_BIAS config) \<longrightarrow>
+                    P (0, (if (\<not> is_unslashed_participating_index val_info TIMELY_TARGET_FLAG_INDEX) 
+                             then (inactivity_score * effective_balance) div
+                                  (INACTIVITY_PENALTY_QUOTIENT_ALTAIR * INACTIVITY_SCORE_BIAS config)
+                          else 0)) s  ))) 
+   (bindCont (get_inactivity_penalty_delta val_info inactivity_score state_ctxt) c)
+   Q "
+  apply (unfold get_inactivity_penalty_delta_def, rule hoare_weaken_pre, wp)
+   apply (clarsimp, fastforce)
+  apply (simp only: if_lift, rule lift_mono')
+  apply (case_tac "\<not> is_unslashed_participating_index val_info TIMELY_TARGET_FLAG_INDEX"; clarsimp simp: Let_unfold)
+  apply (intro conjI)
+  apply (rule safe_mul_not_zeroI)
+  using safe_mul_commute apply blast
+    apply (clarsimp)
+   apply (clarsimp simp: INACTIVITY_PENALTY_QUOTIENT_ALTAIR_def)
+  by (clarsimp simp: mult.commute)
+
+
+lemma read_beacon_wp_ex[wp]: "(\<And>x. hoare_triple ( lift (P x)) (c x) (Q )) \<Longrightarrow> 
+hoare_triple (lift ((EXS v. maps_to l v \<and>* (maps_to l v \<longrightarrow>*  (P v ))))) (do {v <- read_beacon l ; c v}) (Q  )"
+  sorry  apply (wp)
+  done
+
+lemma drop_maps_to_lift: "lift (maps_to l v \<and>* R) s \<Longrightarrow> lift R s"
+  apply (clarsimp simp: lift_def)
+  apply (clarsimp simp: sep_conj_def maps_to_def)
+  apply (rule_tac x=y in exI)
+  apply (clarsimp)
+  apply (clarsimp simp: point_of_plus_domain_iff)
+  by (metis comp_apply point_of_plus_domain_iff sep_add_commute valid_write_write)
+
+find_theorems alloc
+
+lemma "\<lless>\<lambda>s. \<forall>x. P x s\<then> \<ge> (ALLS x. lift (P x))" 
+  apply (clarsimp)
+
+
+  find_theorems lift "\<forall>x. ?P x"
+
+lemma "(\<And>s. lift P s \<Longrightarrow> lift Q s) \<Longrightarrow> lift P \<le> lift Q"
+  sledgehammer
+  by (simp add: le_funI)
+  by blast
+  apply (clarsimp)
+
+lemma case_simplifier_0: "(0 = TIMELY_HEAD_FLAG_INDEX \<longrightarrow> P) = True"
+  by (clarsimp simp: TIMELY_HEAD_FLAG_INDEX_def)
+
+
+lemma case_simplifier_1: "(1 = TIMELY_HEAD_FLAG_INDEX \<longrightarrow> P) = True"
+  by (clarsimp simp: TIMELY_HEAD_FLAG_INDEX_def)
+
+
+lemma case_simplifier_1': "(Suc 0 = TIMELY_HEAD_FLAG_INDEX \<longrightarrow> P) = True"
+  by (clarsimp simp: TIMELY_HEAD_FLAG_INDEX_def)
+
+
+lemma case_simplifier_2: "(2 = TIMELY_HEAD_FLAG_INDEX \<longrightarrow> P) = P"
+  by (clarsimp simp: TIMELY_HEAD_FLAG_INDEX_def)
+
+lemmas case_flag_simplifiers = case_simplifier_0 case_simplifier_1 case_simplifier_2 case_simplifier_1'
+
+definition "assuming P R \<equiv> P \<and> (P \<longrightarrow> R)"
+
+
+lemma write_beacon_wp': "\<lblot>\<lless>P\<then>\<rblot> c () \<lblot>Q\<rblot> \<Longrightarrow> \<lblot>\<lless>(EXS v. l \<mapsto>\<^sub>l v) \<and>* (l \<mapsto>\<^sub>l v' \<longrightarrow>* P)\<then>\<rblot> bindCont (write_to l v') c \<lblot>Q\<rblot>"
+  sorry
+
+lemma maps_exI[sep_cancel]: "(maps_to l v) s \<Longrightarrow> (EXS v. maps_to l v) s"
+  by (blast)
+
+lemma rewardable_is_unslashed[simp]: "rewardable x y z \<Longrightarrow> is_unslashed_participating_index x y"
+  by (clarsimp simp: rewardable_def)
+
+lemma unrewardable_is_slashed: "\<not>rewardable x y z \<Longrightarrow> \<not>is_in_inactivity_leak_f z \<Longrightarrow> \<not>is_unslashed_participating_index x y"
+  by (clarsimp simp: rewardable_def)
+
+
+lemma unrewardable_is_leaking: "\<not>rewardable x y z \<Longrightarrow> is_unslashed_participating_index x y \<Longrightarrow> is_in_inactivity_leak_f z"
+  apply (simp only: rewardable_def)
+  by (clarsimp)
+
+lemmas unrewardable_simps = unrewardable_is_slashed unrewardable_is_leaking
+
+lemma rewardable_not_in_inactivity_leak[simp]: "rewardable x y z \<Longrightarrow> \<not>is_in_inactivity_leak_f z"
+  apply (simp only: rewardable_def)
+  by (clarsimp)
+
+lemma par_index_zero[simp]: "PARTICIPATION_FLAG_WEIGHTS ! 0 = TIMELY_SOURCE_WEIGHT"
+  by (clarsimp simp: PARTICIPATION_FLAG_WEIGHTS_def)
+
+lemma par_index_one[simp]: "PARTICIPATION_FLAG_WEIGHTS ! (Suc 0) = TIMELY_TARGET_WEIGHT"
+  by (clarsimp simp: PARTICIPATION_FLAG_WEIGHTS_def)
+
+
+lemma par_index_two[simp]: "PARTICIPATION_FLAG_WEIGHTS ! 2 = TIMELY_HEAD_WEIGHT"
+  by (clarsimp simp: PARTICIPATION_FLAG_WEIGHTS_def)
+
+lemma sum_bounded_l: "x \<le> x + (y :: u64) \<longleftrightarrow> unat x + unat y < 2 ^ 64"
+  apply (safe)
+   apply (unat_arith, simp)
+  apply (unat_arith, simp)
+  done
+
+lemma sum_bounded_r: "y \<le> x + (y :: u64) \<longleftrightarrow> unat x + unat y < 2 ^ 64"
+  apply (safe)
+   apply (unat_arith, simp)
+  apply (unat_arith, simp)
+  done
+
+lemma unat_plus_distrib_bounded: "unat (x + y) = unat x + unat (y :: u64) \<longleftrightarrow> unat x + unat y < 2 ^ 64"
+  apply (safe)
+   apply (unat_arith, simp)
+  using sum_bounded_l unat_plus_simple by blast
+  apply (unat_arith, simp)
+  done
+
+lemmas sum_bounded = sum_bounded_l sum_bounded_r
+
+lemma chain_safe: "x \<le> x + z \<Longrightarrow> z \<ge> y \<Longrightarrow> x \<le> x + (y :: u64)"
+  by (unat_arith)
+
+lemmas safe_sum_iff = unat_plus_distrib_bounded[THEN iffD2]
+
+
+lemma free_wp[wp]:" \<lblot>\<lless>P ()\<then>\<rblot> c () \<lblot>Q\<rblot> \<Longrightarrow> \<lblot>\<lless>\<lambda>s.  ((EXS v. l \<mapsto>\<^sub>l v) \<and>* P ()) s\<then>\<rblot> (bindCont (free l) c) \<lblot>Q\<rblot>" sorry
+
+
+lemma saturating_sub_simp1[simp]: "b \<le> a \<Longrightarrow> saturating_sub a b = a - b"
+  by (clarsimp simp: saturating_sub_def)
+
+
+lemma saturating_sub_simp2[simp]: "b \<ge> (a :: u64) \<Longrightarrow> saturating_sub a b = 0"
+  by (clarsimp simp: saturating_sub_def)
+
+lemma process_single_reward_and_penalty_wp[wp]: "
+ (\<And>x. hoare_triple (lift (P x)) (c x) Q) \<Longrightarrow>
+  hoare_triple (lift (\<lambda>s. let eff_balance = (ValidatorInfo.effective_balance_f validator_info);
+                              rewards = map (\<lambda>n. if rewardable validator_info n state_ctxt then base_reward_f validator_info * PARTICIPATION_FLAG_WEIGHTS ! n * unslashed_participating_increments_array_f rewards_ctxt ! n div
+                                                                      (active_increments_f rewards_ctxt * WEIGHT_DENOMINATOR) else 0) [0, 1, 2];
+                                          penalties = map (\<lambda>n. if \<not>(rewardable validator_info n state_ctxt) then base_reward_f validator_info * PARTICIPATION_FLAG_WEIGHTS ! n div WEIGHT_DENOMINATOR 
+                                                                                                             else 0) [0,1];
+                                          inactivity_penalty_delta = (if \<not> is_unslashed_participating_index validator_info TIMELY_TARGET_FLAG_INDEX then 
+                                                                           inactivity_score * eff_balance div 
+                                                                           (INACTIVITY_PENALTY_QUOTIENT_ALTAIR * INACTIVITY_SCORE_BIAS config) else 0);
+                                          result = (if is_eligible_f validator_info then saturating_sub (balance + sum_list rewards) (sum_list penalties + inactivity_penalty_delta) else balance)
+                           in  \<forall>n\<in>{0,1,2}. let unslashed_participating_increment = unslashed_participating_increments_array_f rewards_ctxt ! n;
+                                                weight = PARTICIPATION_FLAG_WEIGHTS ! n              
+                                         in n < length PARTICIPATION_FLAG_WEIGHTS \<and>
+                                            n < length (unslashed_participating_increments_array_f rewards_ctxt) \<and>
+                                            balance \<le> balance + sum_list rewards \<and>
+                                            sum_list (map unat rewards) + unat inactivity_penalty_delta  < 2^64 \<and> 
+                                            (sum_list (map unat penalties) + unat inactivity_penalty_delta) < 2 ^ 64 \<and>
+                                            safe_mul weight (base_reward_f validator_info) \<and>
+                                            safe_mul inactivity_score eff_balance \<and>
+                                            safe_mul (weight * base_reward_f validator_info) unslashed_participating_increment \<and>
+                                            safe_mul (active_increments_f rewards_ctxt) WEIGHT_DENOMINATOR \<and>
+                                            safe_mul INACTIVITY_PENALTY_QUOTIENT_ALTAIR (INACTIVITY_SCORE_BIAS config) \<and>
+                                            active_increments_f rewards_ctxt * WEIGHT_DENOMINATOR \<noteq> 0 \<and>
+                                            (n < length PARTICIPATION_FLAG_WEIGHTS \<and> safe_mul inactivity_score eff_balance \<and>
+                                             n < length (unslashed_participating_increments_array_f rewards_ctxt) \<and>
+                                             safe_mul weight (base_reward_f validator_info) \<and> safe_mul INACTIVITY_PENALTY_QUOTIENT_ALTAIR (INACTIVITY_SCORE_BIAS config) \<and>
+                                             safe_mul (weight * base_reward_f validator_info) unslashed_participating_increment \<and>
+                                             safe_mul (active_increments_f rewards_ctxt) WEIGHT_DENOMINATOR \<and> active_increments_f rewards_ctxt * WEIGHT_DENOMINATOR \<noteq> 0 \<longrightarrow> (P (result)) s)))
+  (bindCont (process_single_reward_and_penalty balance inactivity_score validator_info rewards_ctxt state_ctxt) c)
+   Q"
+  apply (unfold process_single_reward_and_penalty_def, rule hoare_weaken_pre, wp)
+    apply (simp only: Let_unfold)
+    apply (clarsimp simp: bindCont_return)
+    apply (simp only: bindCont_assoc[symmetric])
+    apply (rule mapM_wp_foldr'[where g="\<lambda>_. ()"])
+     apply (simp only: bindCont_assoc[symmetric])
+     apply (rule get_flag_index_delta_wp_gen)
+     apply (simp only: bindCont_assoc[symmetric] | rule read_beacon_wp_ex add_wp' write_beacon_wp' wp | fastforce)+
+  apply (simp only: if_lift TIMELY_TARGET_FLAG_INDEX_def TIMELY_HEAD_FLAG_INDEX_def TIMELY_SOURCE_FLAG_INDEX_def)
+  apply (clarsimp)
+   apply (unfold range_participation_flag_weights_simp[simplified])
+   apply (simp only: foldr.simps case_flag_simplifiers)
+  apply (intro conjI impI; clarsimp simp: Let_unfold)
+  apply ( (sep_cancel | intro conjI impI allI | clarsimp simp:  | (rule exI, sep_cancel+) | (erule sep_curry[rotated, where P="P result" for result]))+,
+       (fastforce simp: sum_bounded safe_sum_iff add.assoc | fastforce simp: sum_bounded safe_sum_iff | (rule exI, intro conjI impI) | clarsimp simp: unrewardable_simps )?)+
+  apply (clarsimp simp: unrewardable_simps  )
+  apply ( (sep_cancel | intro conjI impI allI | clarsimp simp:  | (rule exI, sep_cancel+) | (erule sep_curry[rotated, where P="P result" for result]))+,
+       (fastforce simp: sum_bounded safe_sum_iff add.assoc | fastforce simp: sum_bounded safe_sum_iff | (rule exI, intro conjI impI))?)+  
+       apply (clarsimp simp: unrewardable_simps  )
+  apply ( (sep_cancel | intro conjI impI allI | clarsimp simp:  | (rule exI, sep_cancel+) | (erule sep_curry[rotated, where P="P result" for result]))+,
+       (fastforce simp: sum_bounded safe_sum_iff add.assoc | fastforce simp: sum_bounded safe_sum_iff | (rule exI, intro conjI impI))?)+ 
+  apply (case_tac "is_unslashed_participating_index validator_info (Suc 0)"; clarsimp?)
+  by ( (sep_cancel | intro conjI impI allI | clarsimp simp:  | (rule exI, sep_cancel+) | (erule sep_curry[rotated, where P="P result" for result]))+,
+       (fastforce simp: sum_bounded safe_sum_iff add.assoc | fastforce simp: sum_bounded safe_sum_iff | (rule exI, intro conjI impI))?)+ 
+
+
+find_theorems process_single_inactivity_update
+find_theorems process_single_slashing
+
+lemma process_single_inactivity_update_wp'[wp]:
+   "(\<And>x. hoare_triple (lift (P x)) (c x) Q) \<Longrightarrow>
+   hoare_triple (lift (\<lambda>s. let result = (if (is_unslashed_participating_index validator_info TIMELY_TARGET_FLAG_INDEX)
+                                             then (saturating_sub score 1)
+                                             else (score + INACTIVITY_SCORE_BIAS config));
+                               result = (if \<not>(is_in_inactivity_leak_f state_ctxt) 
+                                             then (saturating_sub result (INACTIVITY_SCORE_RECOVERY_RATE config))
+                                             else (result));
+                               result = (if \<not>(is_eligible_f validator_info) then score else result) in
+                               score \<le> score + INACTIVITY_SCORE_BIAS config \<and>  P result s)) 
+    (bindCont (process_single_inactivity_update score validator_info state_ctxt) c) Q"
+  apply (unfold process_single_inactivity_update_def, rule hoare_weaken_pre, wp)
+    apply (fastforce)
+   apply (wp)
+    apply (fastforce)
+   apply (wp)
+   apply (fastforce)
+  apply (clarsimp simp: Let_unfold)
+  apply (intro conjI impI allI; clarsimp simp: saturating_sub_def)
+    apply (intro conjI impI allI; clarsimp simp: saturating_sub_def)
+  apply (intro conjI impI allI; clarsimp simp: saturating_sub_def)
+  apply (intro conjI impI allI; clarsimp simp: saturating_sub_def)
+  done
+
+lemma process_single_slashing[wp]:
+   "(\<And>x. hoare_triple (lift (P x)) (c x) Q) \<Longrightarrow>
+   hoare_triple (lift (\<lambda>s. let effective_balance = Validator.effective_balance_f validator in
+                           let effective_balance_increment = (effective_balance div EFFECTIVE_BALANCE_INCREMENT config) in
+                           let result = (if Validator.slashed_f validator \<and> 
+                                            target_withdrawable_epoch_f slashings_ctxt = withdrawable_epoch_f validator
+                                          then
+                                             saturating_sub balance (effective_balance_increment * adjusted_total_slashing_balance_f slashings_ctxt div total_active_balance_f progressive_balances *
+                                             EFFECTIVE_BALANCE_INCREMENT config)
+                                          else balance) in 
+                        safe_mul (adjusted_total_slashing_balance_f slashings_ctxt) effective_balance_increment \<and>
+                        total_active_balance_f progressive_balances \<noteq> 0  \<and>
+                         safe_mul (EFFECTIVE_BALANCE_INCREMENT config)
+                         (effective_balance_increment * adjusted_total_slashing_balance_f slashings_ctxt div total_active_balance_f progressive_balances) \<and>
+                        
+                         (safe_mul (adjusted_total_slashing_balance_f slashings_ctxt) effective_balance_increment \<and>
+                           total_active_balance_f progressive_balances \<noteq> 0  \<and>
+                           safe_mul (EFFECTIVE_BALANCE_INCREMENT config)
+                          (effective_balance_increment * adjusted_total_slashing_balance_f slashings_ctxt div total_active_balance_f progressive_balances) \<longrightarrow>
+                          P result s)))
+    (bindCont (process_single_slashing balance validator slashings_ctxt progressive_balances) c) Q"
+  apply (unfold process_single_slashing_def, rule hoare_weaken_pre, wp)
+   apply (fastforce)
+  apply (clarsimp simp: ebi_not_zero Let_unfold)
+  apply (intro conjI impI allI; clarsimp simp: saturating_sub_def)
+    apply (intro conjI impI allI; clarsimp simp: saturating_sub_def)
+  done
+
+
+lemma "(P -* P \<and>* R) s \<Longrightarrow> (P -* (P \<and>* (P \<longrightarrow>* (P \<and>* R)))) s"
+  apply (rule septract_cancel[rotated], assumption)
+   apply (rule sep_conj_impl[rotated], assumption)
+    apply (erule sep_curry', assumption, assumption)
+  done
+
+lemma "(P -* P \<and>* R) s \<Longrightarrow> (P -* (P \<and>* (P \<longrightarrow>* R))) s"
+  apply (rule septract_cancel, assumption, assumption)
+  apply (sep_cancel)
+  apply (clarsimp simp: sep_conj_def sep_impl_def)
+  oops
+
+lemma "(P \<and>* R) s \<Longrightarrow> (P \<and>* (P -* P \<and>* R)) s"
+  apply (clarsimp simp: sep_conj_def sep_impl_def septraction_def pred_neg_def)
+  apply (rule_tac x="x" in exI)
+  apply (rule_tac x=y in exI)
+  apply (clarsimp)
+  apply (rule_tac x=x in exI)
+  apply (clarsimp simp: sep_disj_commute)
+  apply (rule_tac x=x in exI, clarsimp)
+  by (metis sep_add_commute)
+
+
+
+
+find_theorems hoare_triple new_rewards_and_penalties_context
+
+lemma septractI_conj: "(\<And>s. Q s \<Longrightarrow> P s) \<Longrightarrow> (\<And>s h. s ## h \<Longrightarrow> P s \<Longrightarrow> \<exists>s'. Q s' \<and> s' ## h) \<Longrightarrow>  (P \<and>* R) s \<Longrightarrow> (P \<and>* (P -* Q \<and>* R)) s"
+  apply (clarsimp simp: septraction_def sep_conj_def sep_impl_def pred_neg_def)
+  sorry
+  apply (rule sep_conj_impl[rotated, where Q="(not (P \<longrightarrow>* not (P \<and>* R)))"], assumption)
+   apply (clarsimp simp: pred_neg_def)
+   apply (erule notE)
+   apply (sep_cancel)
+  apply (sep_mp)
+  apply (rule septract_cancel[rotated])
+  apply (clarsimp simp: sep_conj_def sep_impl_def septraction_def pred_neg_def)
+  apply (rule_tac x="x" in exI)
+  apply (rule_tac x=y in exI)
+  apply (clarsimp)
+  apply (rule_tac x=x in exI)
+  apply (clarsimp simp: sep_disj_commute)
+  apply (rule_tac x=x in exI)
+  oops
+  by (metis sep_add_commute)
+
+lemma maps_to_mutual_disjoint: "maps_to l v s \<Longrightarrow> s ## h \<Longrightarrow> \<exists>s'. maps_to l v' s' \<and> s' ## h"
+  by (metis maps_to_def maps_to_lens_pset' sep_disj_p_set_def)
+
+lemma "\<forall>c P Q . (\<forall>x. hoare_triple (lift (P x \<and>* (EXS n. num_active_validators \<mapsto>\<^sub>l n))) (c x) Q) \<longrightarrow>
+   (\<exists>P.  hoare_triple (lift P) (bindCont get_validator_churn_limit c) Q 
+ \<and> (\<exists>P'. hoare_triple (lift P') (bindCont get_validator_churn_limit_fast c) (Q) \<and> ( P \<le> ((EXS n. num_active_validators \<mapsto>\<^sub>l n) \<and>* ((EXS n. num_active_validators \<mapsto>\<^sub>l n) -* P')))))" 
+  apply (clarsimp)
+  apply (rule exI)
+  apply (intro conjI)
+    apply (rule get_validator_churn_limit_spec')
+  apply (erule_tac x=x in allE)
+    apply (assumption)
+  apply (rule exI)
+  apply (intro conjI)
+   apply (rule get_validator_churn_limit_fast_wp)
+   apply (fastforce)
+  apply (clarsimp)
+  apply (sep_mp)
+  apply (rule septractI_conj, blast)
+    apply (clarsimp)
+  apply (erule (1) maps_to_mutual_disjoint)
+
+  apply (sep_cancel)+
+  apply (blast)
   done
 
 end
